extracting signatures

composed_vlsm.v
@@ -2,20 +2,9 @@ Require Import List.
 Import ListNotations.
 
 From Casper
-Require Import vlsm two_vlsms list_of_vlsms indexed_vlsm.
+Require Import vlsm two_vlsms indexed_vlsm.
 
-
-Definition noneOrAll
-  (op : option Prop)
-  : Prop
-  :=
-  match op with
-  | None => True
-  | (Some p) => p
-  end.
-
-
-Class composed_vlsm_class (message : Type) `{VLSM message} :=
+Class composed_sig_class (message : Type) `{S : LSM_sig message} :=
   { index : Set
   ; index_eq_dec : EqDec index
 
@@ -30,35 +19,18 @@ Class composed_vlsm_class (message : Type) `{VLSM message} :=
   ; iproto_message_decidable : forall i : index, forall m : message, {iproto_message_prop i m} + {~iproto_message_prop i m}
   ; iproto_message_inhabited : forall i : index, inhabited {m : message | iproto_message_prop i m}
   ; iproto_message_consistent : forall i : index, forall m : message, iproto_message_prop i m -> proto_message_prop m
-
-  ; transition_projection_consistency
-    : forall (s1 s2 : state) (om : option proto_message) (l : label) (i : index)
-        (Hproj_s : istate_proj i s1 = istate_proj i s2)
-        (Hli : ilabel l = i),
-    (   snd (transition l (s1, om)) = snd (transition l (s2, om))
-    /\  istate_proj i (fst (transition l (s1, om))) = istate_proj i (fst (transition l (s2, om)))
-    )
-  ; transition_projection_state_preservation
-    : forall (s : state) (om : option proto_message) (l : label) (i : index)
-        (Hnli : ilabel l <> i),
-        (istate_proj i (fst (transition l (s, om))) = istate_proj i s
-    )
-  ; transition_projection_type_preservation
-    : forall (s : state) (om : option proto_message) (l : label) (i : index)
-        (Hli : ilabel l = i),
-        noneOrAll (option_map (iproto_message_prop i) (option_map (@proj1_sig message proto_message_prop) (snd (transition l (s, om)))))
   }.
 
 Definition istate
   { message : Type }
-  `{composed_vlsm_class message}
+  `{composed_sig_class message}
   (i : index)
   :=
   { is : iproto_state i | exists s : state, istate_proj i s = is }.
 
 Definition proj_istate
   { message : Type }
-  `{composed_vlsm_class message}
+  `{composed_sig_class message}
   (s : state)
   (i : index)
   : istate i.
@@ -69,7 +41,7 @@ Defined.
 
 Lemma proj_istate_eq
   { message : Type }
-  `{composed_vlsm_class message}
+  `{composed_sig_class message}
   (s1 s2 : state)
   (i : index)
   : istate_proj i s1 = istate_proj i s2 <-> proj_istate s1 i = proj_istate s2 i.
@@ -79,6 +51,33 @@ Proof.
   - apply exist_eq. simpl. assumption.
   - inversion Heq. reflexivity.
 Qed.
+
+
+Class composed_vlsm_class (message : Type) {S : LSM_sig message} `{@composed_sig_class message S} `{M : @VLSM message S}
+  :=
+  { transition_projection_consistency
+    : forall (s1 s2 : state) (om : option proto_message) (l : label) (i : index := ilabel l)
+        (Hproj_s : istate_proj i s1 = istate_proj i s2),
+      let (s1', om1') := transition l (s1, om) in
+      let (s2', om2') := transition l (s2, om) in
+      om1' = om2' /\  istate_proj i s1' = istate_proj i s2'
+  ; transition_projection_state_preservation
+    : forall (s : state) (om : option proto_message) (l : label) (i : index)
+        (Hnli : ilabel l <> i),
+        let (s', _) := transition l (s, om) in
+        istate_proj i s' = istate_proj i s
+  ; transition_projection_message_type_preservation
+    : forall (s : state) (om : option proto_message) (l : label) (i : index := ilabel l)
+        (s' : state)
+        (m' : proto_message)
+        (Ht : transition l (s, om) = (s', Some m')),
+        (iproto_message_prop i (proj1_sig m'))
+  ; transition_projection_message_type_mismatch
+    : forall (s : state) (m : proto_message) (l : label) (i : index := ilabel l)
+        (Hnm : ~ (iproto_message_prop i (proj1_sig m))),
+        ~ valid l (s, Some m)
+  }.
+
 
 Inductive composed2_index : Set := one | two.
 
@@ -90,8 +89,8 @@ Qed.
 
 Definition composed2_iproto_state
   {message}
-  (S1 : VLSM message)
-  (S2 : VLSM message)
+  (S1 : LSM_sig message)
+  (S2 : LSM_sig message)
   (i : composed2_index)
   : Type
   :=
@@ -102,10 +101,10 @@ Definition composed2_iproto_state
 
 Definition composed2_istate_proj
   {message}
-  (S1 : VLSM message)
-  (S2 : VLSM message)
+  (S1 : LSM_sig message)
+  (S2 : LSM_sig message)
   (i : composed2_index)
-  (s : (@state message S1) * (@state message S2))
+  (s : @state message (composed2_sig S1 S2))
   : composed2_iproto_state S1 S2 i
   :=
   match i with
@@ -113,21 +112,11 @@ Definition composed2_istate_proj
   | two => snd s
   end.
 
-Definition composed2_istate_proj'
-  {message}
-  (S1 : VLSM message)
-  (S2 : VLSM message)
-  (i : composed2_index)
-  (s : @state message (composed2_vlsm S1 S2))
-  : composed2_iproto_state S1 S2 i
-  :=
-  composed2_istate_proj S1 S2 i s.
-
 Definition composed2_ilabel
   {message}
-  (S1 : VLSM message)
-  (S2 : VLSM message)
-  (l : (@label message S1) + (@label message S2))
+  (S1 : LSM_sig message)
+  (S2 : LSM_sig message)
+  (l : @label _ (composed2_sig S1 S2))
   : composed2_index
   :=
   match l with
@@ -137,10 +126,10 @@ Definition composed2_ilabel
 
 Lemma composed2_ilabel_type_inhabited
   {message}
-  (S1 : VLSM message)
-  (S2 : VLSM message)
+  (S1 : LSM_sig message)
+  (S2 : LSM_sig message)
   (i : composed2_index)
-  : inhabited { l : @label message S1 + @label message S2 | composed2_ilabel S1 S2 l = i }.
+  : inhabited { l : @label _ (composed2_sig S1 S2) | composed2_ilabel S1 S2 l = i }.
 Proof.
   specialize (@label_inhabited message S1); intros [l1].
   specialize (@label_inhabited message S2); intros [l2].
@@ -152,8 +141,8 @@ Qed.
 
 Definition composed2_iproto_message_prop
   {message}
-  (S1 : VLSM message)
-  (S2 : VLSM message)
+  (S1 : LSM_sig message)
+  (S2 : LSM_sig message)
   (i : composed2_index)
   : message -> Prop
   :=
@@ -164,8 +153,8 @@ Definition composed2_iproto_message_prop
 
 Lemma composed2_iproto_message_decidable
   {message}
-  (S1 : VLSM message)
-  (S2 : VLSM message)
+  (S1 : LSM_sig message)
+  (S2 : LSM_sig message)
   (i : composed2_index)
   : forall m : message, {composed2_iproto_message_prop S1 S2 i m} + {~composed2_iproto_message_prop S1 S2 i m}.
 Proof.
@@ -174,8 +163,8 @@ Qed.
 
 Lemma composed2_iproto_message_inhabited
   {message}
-  (S1 : VLSM message)
-  (S2 : VLSM message)
+  (S1 : LSM_sig message)
+  (S2 : LSM_sig message)
   (i : composed2_index)
   : inhabited {m : message | composed2_iproto_message_prop S1 S2 i m}.
 Proof.
@@ -184,523 +173,180 @@ Qed.
 
 Lemma composed2_iproto_message_consistent
   {message}
-  (S1 : VLSM message)
-  (S2 : VLSM message)
+  (S1 : LSM_sig message)
+  (S2 : LSM_sig message)
   (i : composed2_index)
-  : forall m : message, composed2_iproto_message_prop S1 S2 i m -> composed2_proto_message_prop S1 S2 m.
+  (m : message)
+  : composed2_iproto_message_prop S1 S2 i m -> composed2_proto_message_prop S1 S2 m.
 Proof.
+  intros Hmsg.
   unfold composed2_iproto_message_prop; intros. destruct i; (left; assumption) || (right; assumption).
 Qed.
 
+Definition composed2_sig_composed_instance
+  {message}
+  (S1 S2 : LSM_sig message)
+  : @composed_sig_class message (composed2_sig S1 S2) :=
+  {| index := composed2_index
+  ; index_eq_dec := composed2_index_eq_dec
+  ; iproto_state := composed2_iproto_state S1 S2
+  ; istate_proj := composed2_istate_proj S1 S2
+  ; ilabel := composed2_ilabel S1 S2
+  ; ilabel_type_inhabited := composed2_ilabel_type_inhabited S1 S2
+  ; iproto_message_prop := composed2_iproto_message_prop S1 S2
+  ; iproto_message_decidable := composed2_iproto_message_decidable S1 S2
+  ; iproto_message_inhabited := composed2_iproto_message_inhabited S1 S2
+  ; iproto_message_consistent := composed2_iproto_message_consistent S1 S2
+  |}.
+
 Lemma composed2_transition_projection_consistency
   {message}
-  (S1 : VLSM message)
-  (S2 : VLSM message)
-  : forall
-      (s1 s2 : @state message S1 * @state message S2)
-      (om : option (composed2_proto_message S1 S2))
-      (l : @label message S1 + @label message S2)
-      (i : composed2_index)
-      (Hproj_s : composed2_istate_proj S1 S2 i s1 = composed2_istate_proj S1 S2 i s2)
-      (Hli : composed2_ilabel S1 S2 l = i),
-    (   snd (composed2_transition S1 S2 l (s1, om)) = snd (composed2_transition S1 S2 l (s2, om))
-    /\  composed2_istate_proj S1 S2 i (fst (composed2_transition S1 S2 l (s1, om)))
-      = composed2_istate_proj S1 S2 i (fst (composed2_transition S1 S2 l (s2, om)))
-    ).
+  {S1 S2 : LSM_sig message}
+  (M1 : @VLSM message S1)
+  (M2 : @VLSM message S2)
+  (s1 s2 : @state _ (composed2_sig S1 S2))
+  (om : option (@proto_message _ (composed2_sig S1 S2)))
+  (l : @label _ (composed2_sig S1 S2))
+  (i : @index _ _ (composed2_sig_composed_instance S1 S2) := composed2_ilabel S1 S2 l)
+  (Hproj_s : composed2_istate_proj S1 S2 i s1 = composed2_istate_proj S1 S2 i s2)
+  : let (s1', om1') := (@transition _ _ (composed2_vlsm M1 M2) l (s1, om)) in
+    let (s2', om2') := (@transition _ _ (composed2_vlsm M1 M2) l (s2, om)) in
+    (   om1' = om2'
+    /\  composed2_istate_proj S1 S2 i s1' = composed2_istate_proj S1 S2 i s2'
+    )
+  .
 Proof.
   intros.
-  destruct s1 as [s1one s1two]. destruct s2 as [s2one s2two].
-  destruct l as [lone | ltwo]; simpl in Hli; subst;  destruct om as [[m Hm]|]; simpl in *; subst; try (split; reflexivity);
-  destruct (proto_message_decidable m) as [Hpm | Hnpm]; simpl; split; reflexivity.
+  destruct s1 as [s1one s1two]. destruct s2 as [s2one s2two]. 
+  unfold transition in *; simpl in *.
+  destruct om as [[m Hm]|]
+  ; destruct l as [lone | ltwo]
+  ; simpl in Hproj_s; subst
+  ; try destruct (proto_message_decidable m) as [Hpm | Hnpm]
+  ; split; reflexivity
+  .
 Qed.
 
 Lemma composed2_transition_projection_state_preservation
   {message}
-  (S1 : VLSM message)
-  (S2 : VLSM message)
-  : forall
-      (s : @state message S1 * @state message S2)
-      (om : option (composed2_proto_message S1 S2))
-      (l : @label message S1 + @label message S2)
-      (i : composed2_index)
-      (Hnli : composed2_ilabel S1 S2 l <> i),
-        composed2_istate_proj S1 S2 i (fst (composed2_transition S1 S2 l (s, om))) = composed2_istate_proj S1 S2 i s
+  {S1 S2 : LSM_sig message}
+  (M1 : @VLSM message S1)
+  (M2 : @VLSM message S2)
+  (s : @state _ (composed2_sig S1 S2))
+  (om : option (@proto_message _ (composed2_sig S1 S2)))
+  (l : @label _ (composed2_sig S1 S2))
+  (i : @index _ _ (composed2_sig_composed_instance S1 S2))
+  (Hnli : @ilabel _ _ (composed2_sig_composed_instance S1 S2) l <> i)
+  : let (s', _) := @transition _ _ (composed2_vlsm M1 M2) l (s, om) in
+    @istate_proj _ _ (composed2_sig_composed_instance S1 S2) i s' = @istate_proj _ _ (composed2_sig_composed_instance S1 S2) i s
   .
 Proof.
   intros.
   destruct s as [sone stwo].
-  destruct i; destruct l as [lone | ltwo]; simpl in Hnli; try contradiction
-  ; destruct om as [[m Hm]|]; try reflexivity
-  ; simpl; destruct (proto_message_decidable m) as [Hpm | Hnpm]
-  ; reflexivity.
+  simpl.
+  destruct om as [[m Hm]|]
+  ; destruct l as [lone | ltwo]
+  ; try destruct (proto_message_decidable m) as [Hpm | Hnpm]
+  ; destruct i;  simpl in Hnli; try contradiction
+  ; reflexivity
+  .
 Qed.
 
-Lemma composed2_transition_projection_type_preservation
+
+Lemma composed2_transition_projection_message_type_mismatch
   {message}
-  (S1 : VLSM message)
-  (S2 : VLSM message)
-  : forall
-      (s : @state message S1 * @state message S2)
-      (om : option (composed2_proto_message S1 S2))
-      (l : @label message S1 + @label message S2)
-      (i : composed2_index)
-      (Hli : composed2_ilabel S1 S2 l = i),
-      noneOrAll
-        (option_map (composed2_iproto_message_prop S1 S2 i)
-          (option_map (@proj1_sig message (composed2_proto_message_prop S1 S2))
-            (snd (composed2_transition S1 S2 l (s, om)))))
-  .
+  {S1 S2 : LSM_sig message}
+  (M1 : @VLSM message S1)
+  (M2 : @VLSM message S2)
+  (s : @state _ (composed2_sig S1 S2))
+  (m : @proto_message _ (composed2_sig S1 S2))
+  (l : @label _ (composed2_sig S1 S2))
+  (i : composed2_index := composed2_ilabel S1 S2 l)
+  (Hnm : ~ (composed2_iproto_message_prop S1 S2 i (proj1_sig m)))
+  : ~ @valid _ _ (composed2_vlsm M1 M2)  l (s, Some m).
 Proof.
-  intros.
-  destruct s as [sone stwo]. destruct l as [lone | ltwo]; simpl in Hli; subst; destruct om as [[m Hm]|]; simpl in *; subst
-  ; try (destruct (proto_message_decidable m) as [Hpm | Hnpm]; simpl); try exact I.
-  - remember (transition lone (sone, Some (exist proto_message_prop m Hpm))) as t.
-    destruct t as (s', om'). destruct om' as [[m' Hpm']|]; simpl; try assumption; try exact I.
-  - remember (transition lone (sone, None)) as t.
-    destruct t as (s', om'). destruct om' as [[m' Hpm']|]; simpl; try assumption; try exact I.
-  - remember (transition ltwo (stwo, Some (exist proto_message_prop m Hpm))) as t.
-    destruct t as (s', om'). destruct om' as [[m' Hpm']|]; simpl; try assumption; try exact I.
-  - remember (transition ltwo (stwo, None)) as t.
-    destruct t as (s', om'). destruct om' as [[m' Hpm']|]; simpl; try assumption; try exact I.
+  simpl. destruct s as [s1 s2]. destruct m as [m Hm].
+  destruct l as [lone | ltwo]
+  ; destruct (proto_message_decidable m)
+  ; intro; contradiction.
+Qed.
+
+
+Lemma composed2_transition_projection_message_type_preservation
+  {message}
+  {S1 S2 : LSM_sig message}
+  (M1 : @VLSM message S1)
+  (M2 : @VLSM message S2)
+  (s : @state _ (composed2_sig S1 S2))
+  (om : option (@proto_message _ (composed2_sig S1 S2)))
+  (l : @label _ (composed2_sig S1 S2))
+  (i : composed2_index := composed2_ilabel S1 S2 l)
+  (s' : @state _ (composed2_sig S1 S2))
+  (m' : @proto_message _ (composed2_sig S1 S2))
+  (Ht : @transition _ _ (composed2_vlsm M1 M2) l (s, om) = (s', Some m'))
+  : composed2_iproto_message_prop S1 S2 i (proj1_sig m').
+Proof.
+  unfold composed2_iproto_message_prop.
+  destruct (transition l (s, om)) as [s'' om'] eqn:Ht'.
+  inversion Ht; subst; clear Ht.
+  simpl in Ht'.
+  destruct s as [s1 s2]. destruct om as [[m Hm]|]
+  ; destruct l as [lone | ltwo]; simpl in i; unfold i
+  ; try destruct (proto_message_decidable m)
+  ; inversion Ht' as [[Hs' Hm']]; subst; clear Ht'
+  .
+  - destruct (transition lone (s1, Some (exist proto_message_prop m p))) as [s'' [[m'' Hm'']|]]; inversion Hm'; subst; assumption.
+  - destruct (transition ltwo (s2, Some (exist proto_message_prop m p))) as [s'' [[m'' Hm'']|]]; inversion Hm'; subst; assumption.
+  - destruct (transition lone (s1, None)) as [s'' [[m'' Hm'']|]]; inversion Hm'; subst; assumption.
+  - destruct (transition ltwo (s2, None)) as [s'' [[m'' Hm'']|]]; inversion Hm'; subst; assumption.
 Qed.
 
 Definition composed2_vlsm_composed_instance
   {message}
-  (S1 : VLSM message)
-  (S2 : VLSM message)
-  : @composed_vlsm_class message (composed2_vlsm S1 S2) :=
-  {| index := composed2_index
-  ; index_eq_dec := composed2_index_eq_dec
-  ; iproto_state := composed2_iproto_state S1 S2
-  ; istate_proj := composed2_istate_proj' S1 S2
-  ; ilabel := composed2_ilabel S1 S2
-  ; ilabel_type_inhabited := composed2_ilabel_type_inhabited S1 S2
-  ; iproto_message_prop := composed2_iproto_message_prop S1 S2
-  ; iproto_message_decidable := composed2_iproto_message_decidable S1 S2
-  ; iproto_message_inhabited := composed2_iproto_message_inhabited S1 S2
-  ; iproto_message_consistent := composed2_iproto_message_consistent S1 S2
-  ; transition_projection_consistency := composed2_transition_projection_consistency S1 S2
-  ; transition_projection_state_preservation := composed2_transition_projection_state_preservation S1 S2
-  ; transition_projection_type_preservation := composed2_transition_projection_type_preservation S1 S2
+  {S1 S2 : LSM_sig message}
+  (M1 : @VLSM message S1)
+  (M2 : @VLSM message S2)
+  : @composed_vlsm_class message _ (@composed2_sig_composed_instance _ S1 S2) (composed2_vlsm M1 M2) :=
+  {| transition_projection_consistency := composed2_transition_projection_consistency M1 M2
+  ; transition_projection_state_preservation := composed2_transition_projection_state_preservation M1 M2
+  ; transition_projection_message_type_mismatch := composed2_transition_projection_message_type_mismatch M1 M2
+  ; transition_projection_message_type_preservation := composed2_transition_projection_message_type_preservation M1 M2
   |}.
 
-Definition composed2_constrained_istate_proj
-  {message}
-  (S1 : VLSM message)
-  (S2 : VLSM message)
-  (constraint : (@label message S1) + (@label message S2) -> (@state message S1 * @state message S2) * option (composed2_proto_message S1 S2) -> Prop)
-  (i : composed2_index)
-  (s : @state message (composed2_vlsm_constrained S1 S2 constraint))
-  : composed2_iproto_state S1 S2 i
-  :=
-  composed2_istate_proj S1 S2 i s.
 
-
-Definition composed2_vlsm_constrained_composed_instance
-  {message}
-  (S1 : VLSM message)
-  (S2 : VLSM message)
-  (constraint : (@label message S1) + (@label message S2) -> (@state message S1 * @state message S2) * option (composed2_proto_message S1 S2) -> Prop)
-  : @composed_vlsm_class message (composed2_vlsm_constrained S1 S2 constraint) :=
-  {| index := composed2_index
-  ; index_eq_dec := composed2_index_eq_dec
-  ; iproto_state := composed2_iproto_state S1 S2
-  ; istate_proj := composed2_constrained_istate_proj S1 S2 constraint
-  ; ilabel := composed2_ilabel S1 S2
-  ; ilabel_type_inhabited := composed2_ilabel_type_inhabited S1 S2
-  ; iproto_message_prop := composed2_iproto_message_prop S1 S2
-  ; iproto_message_decidable := composed2_iproto_message_decidable S1 S2
-  ; iproto_message_inhabited := composed2_iproto_message_inhabited S1 S2
-  ; iproto_message_consistent := composed2_iproto_message_consistent S1 S2
-  ; transition_projection_consistency := composed2_transition_projection_consistency S1 S2
-  ; transition_projection_state_preservation := composed2_transition_projection_state_preservation S1 S2
-  ; transition_projection_type_preservation := composed2_transition_projection_type_preservation S1 S2
-  |}.
-
-Definition composed_list_index
-  {message}
-  (Ss : list (VLSM message))
-  :=
-  { n : nat | n < length Ss }.
-
-Lemma composed_list_index_eq_dec
-  {message}
-  (Ss : list (VLSM message))
- : EqDec (composed_list_index Ss).
-Proof.
-  apply DepEqDec. apply nat_eq_dec.
-Qed.
-
-Fixpoint composed_list_iproto_state
-  {message}
-  (Ss : list (VLSM message))
-  (i : composed_list_index Ss)
-  : Type.
-destruct i as [i Hi].
-destruct Ss as [| Sh St]; simpl in Hi.
-{ exfalso. inversion Hi. }
-destruct i.
-- exact (@state message Sh).
-- apply le_pred in Hi; simpl in Hi.
-  exact (composed_list_iproto_state message St (exist _ i Hi)).
-Defined.
-
-Fixpoint composed_list_istate_proj
-  {message}
-  (Ss : list (VLSM message))
-  (i : composed_list_index Ss)
-  : composed_list_state Ss -> composed_list_iproto_state Ss i.
-intros s.
-destruct i as [i Hi]. 
-destruct Ss as [| Sh St]; simpl in Hi; simpl.
-{ exfalso. inversion Hi. }
-destruct s as [sh st]; simpl.
-destruct i.
-- exact sh.
-- remember (exist (fun n : nat => n < length St) i (le_pred (S (S i)) (S (length St)) Hi)) as i'.
-  exact (composed_list_istate_proj message St i' st).
-Defined.
-
-Definition composed_list_istate_proj'
-  {message}
-  (Ss : list (VLSM message))
-  (Ssnn : Ss <> [])
-  (i : composed_list_index Ss)
-  (s : @state message (composed_list_vlsm Ss Ssnn))
-  : composed_list_iproto_state Ss i
-  := composed_list_istate_proj Ss i s.
-
-
-Definition composed_list_ilabel
-  {message}
-  (Ss : list (VLSM message))
-  (l : composed_list_label Ss)
-  : composed_list_index Ss.
-induction Ss; try contradiction.
-destruct l as [lh | lt].
-- assert (Hi : 0 < length (a :: Ss)) by (apply le_n_S; apply le_0_n).
-  exact (exist _ 0 Hi).
-- specialize (IHSs  lt).
-  destruct IHSs as [i Hi]. apply  le_n_S in Hi.
-  exact (exist _ (S i) Hi).
-Defined.
-
-Lemma composed_list_ilabel_type_inhabited
-  {message}
-  (Ss : list (VLSM message))
-  (i : composed_list_index Ss)
-  : inhabited { l : composed_list_label Ss | composed_list_ilabel Ss l = i }.
-Proof.
-  induction Ss as [| Sh St IHSt]; destruct i as [i Hi].
-  - exfalso. inversion Hi.
-  - destruct i.
-    + specialize (@label_inhabited message Sh); intros [lh].
-      constructor. exists (inl lh). simpl. apply f_equal. apply proof_irrelevance.
-    + simpl in Hi. specialize (IHSt (exist _ i (le_pred _ _ Hi))).
-      destruct IHSt as [[lt Hlt]].
-      constructor.
-      exists (inr lt).
-      simpl. rewrite Hlt. apply f_equal. apply proof_irrelevance.
-Qed.
-
-Fixpoint composed_list_iproto_message_prop
-  {message}
-  (Ss : list (VLSM message))
-  : composed_list_index Ss -> message -> Prop.
-intros [i Hi] m.
-destruct Ss as [| Sh St].
-- exfalso. inversion Hi.
-- destruct i.
-  + exact (@proto_message_prop message Sh m).
-  + specialize (composed_list_iproto_message_prop message St).
-    specialize (composed_list_iproto_message_prop (exist _ i (le_pred _ _ Hi))).
-    exact (composed_list_iproto_message_prop m).
-Defined.
-
-Lemma composed_list_iproto_message_decidable
-  {message}
-  (Ss : list (VLSM message))
-  (i : composed_list_index Ss)
-  : forall m : message, {composed_list_iproto_message_prop Ss i m} + {~composed_list_iproto_message_prop Ss i m}.
-Proof.
-  induction Ss; destruct i as [i Hi].
-  - exfalso. inversion Hi.
-  - destruct i; simpl; try apply proto_message_decidable.
-    specialize (IHSs  (exist _ i (le_pred _ _ Hi))); simpl in IHSs.
-    assumption.
-Qed.
-
-Lemma composed_list_iproto_message_inhabited
-  {message}
-  (Ss : list (VLSM message))
-  (i : composed_list_index Ss)
-  : inhabited {m : message | composed_list_iproto_message_prop Ss i m}.
-Proof.
-  induction Ss; destruct i as [i Hi].
-  - exfalso. inversion Hi.
-  - destruct i; simpl; try apply message_inhabited.
-    specialize (IHSs  (exist _ i (le_pred _ _ Hi))); simpl in IHSs.
-    assumption.
-Qed.
-
-Lemma composed_list_iproto_message_consistent
-  {message}
-  (Ss : list (VLSM message))
-  (i : composed_list_index Ss)
-  : forall m : message, composed_list_iproto_message_prop Ss i m -> composed_list_proto_message_prop Ss m.
-Proof.
-  induction Ss; destruct i as [i Hi].
-  - exfalso. inversion Hi.
-  - destruct i; simpl; intros.
-    + left. assumption.
-    + right. specialize (IHSs (exist _ i (le_pred _ _ Hi)) m). simpl in IHSs.
-      apply IHSs. assumption.
-Qed.
-
-Lemma composed_list_transition_projection_consistency
-  {message}
-  (Ss : list (VLSM message))
-  : forall
-      (s1 s2 : composed_list_state Ss)
-      (om : option (composed_list_proto_message Ss))
-      (l : composed_list_label Ss)
-      (i : composed_list_index Ss)
-      (Hproj_s : composed_list_istate_proj Ss i s1 = composed_list_istate_proj Ss i s2)
-      (Hli : composed_list_ilabel Ss l = i),
-    (   snd (composed_list_transition Ss l (s1, om)) = snd (composed_list_transition Ss l (s2, om))
-    /\  composed_list_istate_proj Ss i (fst (composed_list_transition Ss l (s1, om)))
-      = composed_list_istate_proj Ss i (fst (composed_list_transition Ss l (s2, om)))
-    ).
-Proof.
-  induction Ss; intros; try contradiction.
-  destruct s1 as [s1h s1t]. destruct s2 as [s2h s2t].
-  destruct i as [i Hi]. destruct i.
-  - simpl in Hproj_s. subst.
-    destruct l as [lh | lt].
-    + simpl.  destruct om as [[m Hm]|]; simpl; try (split; reflexivity).
-      destruct (proto_message_decidable m) as [Hpm | Hnpm]; simpl; split; reflexivity.
-    + simpl in Hli. destruct (composed_list_ilabel Ss lt) as [j Hj] eqn:Hl. inversion Hli.
-  - simpl in Hproj_s. simpl in Hi.
-    destruct l as [lh | lt].
-    +  simpl in Hli. inversion Hli.
-    + destruct om as [[m Hm]|].
-      * simpl. destruct (composed_list_proto_message_decidable Ss m) as [Hpm | Hnpm]; simpl; try (split; reflexivity || assumption).
-        specialize (IHSs s1t s2t (Some (exist _ m Hpm)) lt (exist _ i (le_pred _ _ Hi)) Hproj_s).
-        simpl in Hli.
-        remember (composed_list_ilabel Ss lt) as j.
-        destruct j as [j Hj].
-        inversion Hli; subst.
-        assert
-          (Hirrelevant :
-            exist (fun n : nat => n < length Ss) i Hj =
-            exist (fun n : nat => n < length Ss) i (le_pred (S (S i)) (S (length Ss)) Hi)
-          ) by ( apply f_equal; apply proof_irrelevance ).
-        specialize (IHSs Hirrelevant).
-        destruct IHSs as [Hmsg' Hs'].
-        split; try assumption. simpl. apply f_equal. assumption.
-      * specialize (IHSs s1t s2t None lt (exist _ i (le_pred _ _ Hi)) Hproj_s).
-        simpl in Hli. 
-        remember (composed_list_ilabel Ss lt) as j.
-        destruct j as [j Hj].
-        inversion Hli; subst.
-        assert
-          (Hirrelevant :
-            exist (fun n : nat => n < length Ss) i Hj =
-            exist (fun n : nat => n < length Ss) i (le_pred (S (S i)) (S (length Ss)) Hi)
-          ) by ( apply f_equal; apply proof_irrelevance ).
-        specialize (IHSs Hirrelevant).
-        destruct IHSs as [Hmsg' Hs'].
-        split; try assumption. simpl. apply f_equal. assumption.
-Qed.
-
-
-Lemma composed_list_transition_projection_state_preservation
-  {message}
-  (Ss : list (VLSM message))
-  : forall
-      (s : composed_list_state Ss)
-      (om : option (composed_list_proto_message Ss))
-      (l : composed_list_label Ss)
-      (i : composed_list_index Ss)
-      (Hnli : composed_list_ilabel Ss l <> i),
-        composed_list_istate_proj Ss i (fst (composed_list_transition Ss l (s, om))) = composed_list_istate_proj Ss i s
-  .
-Proof.
-  induction Ss as [| Sh St IHSt]; intros; try contradiction.
-  destruct s as [sh st].
-  destruct i as [i Hi]. destruct i; destruct l as [lh |lt]
-  ; destruct om as [[m Hm]|]; try reflexivity
-  ; simpl in Hnli
-  ; try (exfalso; apply Hnli; apply f_equal; apply proof_irrelevance); simpl.
-  - destruct (composed_list_proto_message_decidable St m) as [Hpm | Hnpm]; simpl; reflexivity.
-  - destruct (proto_message_decidable m) as [Hpm | Hnpm]; simpl; reflexivity.
-  - destruct (composed_list_proto_message_decidable St m) as [Hpm | Hnpm]; simpl; try reflexivity.
-    specialize (IHSt st (Some (exist _ m Hpm)) lt (exist _ i (le_pred _ _ Hi))).
-    simpl in IHSt. apply IHSt.
-    remember (composed_list_ilabel St lt) as j. destruct j as [j Hj].
-    intros Heq. apply Hnli. inversion Heq; subst. apply f_equal. apply proof_irrelevance.
-  - specialize (IHSt st None lt (exist _ i (le_pred _ _ Hi))).
-    simpl in IHSt. apply IHSt.
-    remember (composed_list_ilabel St lt) as j. destruct j as [j Hj].
-    intros Heq. apply Hnli. inversion Heq; subst. apply f_equal. apply proof_irrelevance.
-Qed.
-
-Lemma composed_list_transition_projection_type_preservation
-  {message}
-  (Ss : list (VLSM message))
-  : forall
-      (s : composed_list_state Ss)
-      (om : option (composed_list_proto_message Ss))
-      (l : composed_list_label Ss)
-      (i : composed_list_index Ss)
-      (Hli : composed_list_ilabel Ss l = i),
-      noneOrAll
-        (option_map (composed_list_iproto_message_prop Ss i)
-          (option_map (@proj1_sig message (composed_list_proto_message_prop Ss))
-            (snd (composed_list_transition Ss l (s, om)))))
-  .
-Proof.
-  induction Ss as [| Sh St IHSt]; intros; try contradiction.
-  destruct s as [sh st].
-  destruct i as [i Hi]. destruct i.
-  - destruct l as [lh | lt].
-    + destruct om as [[m Hm]|]; simpl in *; subst
-      ; try (destruct (proto_message_decidable m) as [Hpm | Hnpm]; simpl); try exact I.
-      * remember (transition lh (sh, Some (exist proto_message_prop m Hpm))) as t.
-        destruct t as (s', om'). destruct om' as [[m' Hpm']|]; simpl; try assumption; try exact I.
-      * remember (transition lh (sh, None)) as t.
-        destruct t as (s', om'). destruct om' as [[m' Hpm']|]; simpl; try assumption; try exact I.
-    + simpl in Hli. destruct (composed_list_ilabel St lt). inversion Hli.
-  - simpl in Hli. destruct l as [lh | lt].
-    + inversion Hli.
-    + destruct om as [[m Hm]|]; simpl in *; subst.
-      * destruct (composed_list_proto_message_decidable St m) as [Hpm | Hnpm]; simpl; try exact I.
-        specialize (IHSt st (Some (exist _ m Hpm)) lt (exist _ i (le_pred _ _ Hi))).
-
-        remember (composed_list_ilabel St lt) as it. destruct it as [it Hit].
-        inversion Hli. subst.
-        assert
-          (Hirrelevant :
-            exist (fun n : nat => n < length St) i Hit =
-            exist (fun n : nat => n < length St) i (le_pred (S (S i)) (S (length St)) Hi)
-          ) by ( apply f_equal; apply proof_irrelevance ).
-        specialize (IHSt Hirrelevant).
-
-
-        remember (Some (exist (composed_list_proto_message_prop St) m Hpm)) as opm.
-        unfold composed_list_state in IHSt. unfold composed_list_proto_message in IHSt.
-        remember (composed_list_transition St lt (st, opm)) as t.
-        destruct t as (s', om'). destruct om' as [[m' Hpm']|]; simpl; try assumption; try exact I.
-      * specialize (IHSt st None lt (exist _ i (le_pred _ _ Hi))).
-
-        remember (composed_list_ilabel St lt) as it. destruct it as [it Hit].
-        inversion Hli. subst.
-        assert
-          (Hirrelevant :
-            exist (fun n : nat => n < length St) i Hit =
-            exist (fun n : nat => n < length St) i (le_pred (S (S i)) (S (length St)) Hi)
-          ) by ( apply f_equal; apply proof_irrelevance ).
-        specialize (IHSt Hirrelevant).
-
-        unfold composed_list_state in IHSt. 
-        remember (composed_list_transition St lt (st, None)) as t.
-        destruct t as (s', om'). destruct om' as [[m' Hpm']|]; simpl; try assumption; try exact I.
-Qed.
-
-Definition composed_list_vlsm_composed_instance
-  {message}
-  (Ss : list (VLSM message))
-  (Ssnn : Ss <> [])
-  : @composed_vlsm_class message (composed_list_vlsm Ss Ssnn) :=
-  {| index := composed_list_index Ss
-  ; index_eq_dec := composed_list_index_eq_dec Ss
-  ; iproto_state := composed_list_iproto_state Ss
-  ; istate_proj := composed_list_istate_proj' Ss Ssnn
-  ; ilabel := composed_list_ilabel Ss
-  ; ilabel_type_inhabited := composed_list_ilabel_type_inhabited Ss
-  ; iproto_message_prop := composed_list_iproto_message_prop Ss
-  ; iproto_message_decidable := composed_list_iproto_message_decidable Ss
-  ; iproto_message_inhabited := composed_list_iproto_message_inhabited Ss
-  ; iproto_message_consistent := composed_list_iproto_message_consistent Ss
-  ; transition_projection_consistency := composed_list_transition_projection_consistency Ss
-  ; transition_projection_state_preservation := composed_list_transition_projection_state_preservation Ss
-  ; transition_projection_type_preservation := composed_list_transition_projection_type_preservation Ss
-  |}.
-
-Definition composed_list_constrained_istate_proj
-  {message}
-  (Ss : list (VLSM message))
-  (Ssnn : Ss <> [])
-  (constraint : composed_list_label Ss -> composed_list_state Ss * option (composed_list_proto_message Ss) -> Prop)
-  (i : composed_list_index Ss)
-  (s : @state message (composed_list_vlsm_constrained Ss Ssnn constraint))
-  : composed_list_iproto_state Ss i
-  := composed_list_istate_proj Ss i s.
-
-
-Definition composed_list_vlsm_constrained_composed_instance
-  {message}
-  (Ss : list (VLSM message))
-  (Ssnn : Ss <> [])
-  (constraint : composed_list_label Ss -> composed_list_state Ss * option (composed_list_proto_message Ss) -> Prop)
-  : @composed_vlsm_class message (composed_list_vlsm_constrained Ss Ssnn constraint) :=
-  {| index := composed_list_index Ss
-  ; index_eq_dec := composed_list_index_eq_dec Ss
-  ; iproto_state := composed_list_iproto_state Ss
-  ; istate_proj := composed_list_constrained_istate_proj Ss Ssnn constraint
-  ; ilabel := composed_list_ilabel Ss
-  ; ilabel_type_inhabited := composed_list_ilabel_type_inhabited Ss
-  ; iproto_message_prop := composed_list_iproto_message_prop Ss
-  ; iproto_message_decidable := composed_list_iproto_message_decidable Ss
-  ; iproto_message_inhabited := composed_list_iproto_message_inhabited Ss
-  ; iproto_message_consistent := composed_list_iproto_message_consistent Ss
-  ; transition_projection_consistency := composed_list_transition_projection_consistency Ss
-  ; transition_projection_state_preservation := composed_list_transition_projection_state_preservation Ss
-  ; transition_projection_type_preservation := composed_list_transition_projection_type_preservation Ss
-  |}.
-
-Definition indexed_vlsm_istate
+Definition indexed_istate
   {oindex : Set} {message : Type} `{Heqd : EqDec oindex}
-  {IS : oindex -> VLSM message}
+  {IS : oindex -> LSM_sig message}
   (i : oindex)
   : Type
   := @state message (IS i).
 
 
-Definition indexed_vlsm_istate_proj
+Definition indexed_istate_proj
   {oindex : Set} {message : Type} `{Heqd : EqDec oindex}
-  {IS : oindex -> VLSM message}
+  {IS : oindex -> LSM_sig message}
+  {Hinh : inhabited oindex}
   (i : oindex)
-  (s : indexed_state IS)
-  : @indexed_vlsm_istate oindex message Heqd IS i
+  (s : @state message (indexed_sig IS Hinh))
+  : @indexed_istate oindex message Heqd IS i
   :=
   s i.
 
-Definition indexed_vlsm_istate_proj'
-  {oindex : Set} {message : Type} `{Heqd : EqDec oindex}
-  {IS : oindex -> VLSM message}
-  {Hi : inhabited oindex}
-  (i : oindex)
-  (s : @state _ (indexed_vlsm IS Hi))
-  : @indexed_vlsm_istate oindex message Heqd IS i
-  :=
-  indexed_vlsm_istate_proj i s.
 
-
-Definition indexed_vlsm_ilabel
+Definition indexed_ilabel
   {oindex : Set} {message : Type} `{Heqd : EqDec oindex}
-  {IS : oindex -> VLSM message}
+  {IS : oindex -> LSM_sig message}
   (l : indexed_label IS)
   : oindex
   :=
   projT1 l.
 
 
-Lemma indexed_vlsm_ilabel_type_inhabited
+Lemma indexed_ilabel_type_inhabited
   {oindex : Set} {message : Type} `{Heqd : EqDec oindex}
-  {IS : oindex -> VLSM message}
+  {IS : oindex -> LSM_sig message}
   (i : oindex)
-  : inhabited { l : indexed_label IS | indexed_vlsm_ilabel l = i }.
+  : inhabited { l : indexed_label IS | indexed_ilabel l = i }.
 Proof.
   specialize (@label_inhabited message (IS i)); intros [li].
   constructor. 
@@ -708,177 +354,174 @@ Proof.
   reflexivity.
 Qed.
 
-Definition indexed_vlsm_iproto_message_prop
+Definition indexed_iproto_message_prop
   {oindex : Set} {message : Type} `{Heqd : EqDec oindex}
-  {IS : oindex -> VLSM message}
+  {IS : oindex -> LSM_sig message}
   (i : oindex)
   : message -> Prop
   :=
   @proto_message_prop message (IS i).
 
-Definition indexed_vlsm_iproto_message_decidable
+Definition indexed_iproto_message_decidable
   {oindex : Set} {message : Type} `{Heqd : EqDec oindex}
-  {IS : oindex -> VLSM message}
+  {IS : oindex -> LSM_sig message}
   (i : oindex)
-  : forall m : message, {indexed_vlsm_iproto_message_prop i m} + {~indexed_vlsm_iproto_message_prop i m}
+  : forall m : message, {indexed_iproto_message_prop i m} + {~indexed_iproto_message_prop i m}
   :=
   @proto_message_decidable message (IS i).
 
-Definition indexed_vlsm_iproto_message_inhabited
+Definition indexed_iproto_message_inhabited
   {oindex : Set} {message : Type} `{Heqd : EqDec oindex}
-  {IS : oindex -> VLSM message}
+  {IS : oindex -> LSM_sig message}
   (i : oindex)
-  : inhabited {m : message | indexed_vlsm_iproto_message_prop i m}
+  : inhabited {m : message | indexed_iproto_message_prop i m}
   :=
   @message_inhabited message (IS i).
 
-Lemma indexed_vlsm_iproto_message_consistent
+Lemma indexed_iproto_message_consistent
   {index : Set} {message : Type} `{Heqd : EqDec index}
-  {IS : index -> VLSM message}
+  {IS : index -> LSM_sig message}
   (i : index)
-  : forall m : message,
-  indexed_vlsm_iproto_message_prop i m ->
-  @proto_message_prop message (indexed_vlsm IS (inhabits i)) m.
+  (m : message)
+  : indexed_iproto_message_prop i m -> indexed_proto_message_prop IS m.
 Proof.
-  unfold indexed_vlsm_iproto_message_prop.
-  intros m Hmi.
-  exists i. assumption.
+  unfold indexed_iproto_message_prop.
+  intros Hmsg. exists i. assumption.
 Qed.
 
-Lemma indexed_vlsm_transition_projection_consistency
+Definition indexed_sig_composed_instance
   {oindex : Set} {message : Type} `{Heqd : EqDec oindex}
-  {IS : oindex -> VLSM message}
-  : forall
-      (s1 s2 : indexed_state IS)
-      (om : option (indexed_proto_message IS))
-      (l : indexed_label IS)
-      (i : oindex)
-      (Hproj_s : indexed_vlsm_istate_proj i s1 = indexed_vlsm_istate_proj i s2)
-      (Hli : indexed_vlsm_ilabel l = i),
-    (   snd (indexed_transition IS l (s1, om)) = snd (indexed_transition IS l (s2, om))
-    /\  indexed_vlsm_istate_proj i (fst (indexed_transition IS l (s1, om)))
-      = indexed_vlsm_istate_proj i (fst (indexed_transition IS l (s2, om)))
-    ).
-Proof.
-  intros.
-  destruct l as [j l]. simpl in Hli. subst.
-  unfold indexed_vlsm_istate_proj in Hproj_s.
-  unfold indexed_vlsm_istate_proj.
-  simpl.
-  destruct om as [[m Hm]|].
-  - destruct (proto_message_decidable m) as [Hpm | Hnpm]; simpl; try (split; reflexivity || assumption).
-    rewrite <- Hproj_s. 
-    remember (transition l (s1 i, Some (exist proto_message_prop m Hpm))) as t.
-    destruct t as [si' om']. simpl. split; try reflexivity.
-    destruct (eq_dec i i); try contradiction.
-    reflexivity.
-  - rewrite <- Hproj_s.
-    remember (transition l (s1 i, None)) as t.
-    destruct t as [si' om']. simpl. split; try reflexivity.
-    destruct (eq_dec i i); try contradiction.
-    reflexivity.
-Qed.
+  (IS : oindex -> LSM_sig message)
+  (Hinh : inhabited oindex)
+  : @composed_sig_class message (indexed_sig IS Hinh) :=
+  {| index := oindex
+  ; iproto_state := @indexed_istate oindex message Heqd IS
+  ; istate_proj := indexed_istate_proj
+  ; ilabel := indexed_ilabel
+  ; ilabel_type_inhabited := indexed_ilabel_type_inhabited
+  ; iproto_message_prop := indexed_iproto_message_prop
+  ; iproto_message_decidable := indexed_iproto_message_decidable
+  ; iproto_message_inhabited := indexed_iproto_message_inhabited
+  ; iproto_message_consistent := indexed_iproto_message_consistent
+  |}.
 
-Lemma indexed_vlsm_transition_projection_state_preservation
+
+
+Lemma indexed_transition_projection_consistency
   {oindex : Set} {message : Type} `{Heqd : EqDec oindex}
-  {IS : oindex -> VLSM message}
-  : forall
-      (s : indexed_state IS)
-      (om : option (indexed_proto_message IS))
-      (l : indexed_label IS)
-      (i : oindex)
-      (Hnli : indexed_vlsm_ilabel l <> i),
-        indexed_vlsm_istate_proj i (fst (indexed_transition IS l (s, om))) = indexed_vlsm_istate_proj i s
+  {IS : oindex -> LSM_sig message}
+  {IM : forall i : oindex, @VLSM message (IS i)}
+  {Hinh : inhabited oindex}
+  (s1 s2 : @state _ (indexed_sig IS Hinh))
+  (om : option (@proto_message _ (indexed_sig IS Hinh)))
+  (l : @label _ (indexed_sig IS Hinh))
+  (i : oindex := @ilabel _ _ (indexed_sig_composed_instance IS Hinh) l)
+  (Hproj_s : @istate_proj _ _ (indexed_sig_composed_instance IS Hinh) i s1 = @istate_proj _ _ (indexed_sig_composed_instance IS Hinh) i s2)
+  : let (s1', om1') := @transition _ _ (indexed_vlsm IM Hinh) l (s1, om) in
+    let (s2', om2') := @transition _ _ (indexed_vlsm IM Hinh) l (s2, om) in
+    (   om1' = om2'
+    /\  @istate_proj _ _ (indexed_sig_composed_instance IS Hinh) i s1' = @istate_proj _ _ (indexed_sig_composed_instance IS Hinh) i s2'
+    )
   .
 Proof.
-  intros.
+  simpl.  destruct l as [j l]. simpl in i. unfold i in *.
+  unfold istate_proj in Hproj_s; simpl in Hproj_s. unfold indexed_istate_proj in *. rewrite Hproj_s.
+  destruct om as [[m Hm]|]
+  ; ( destruct (proto_message_decidable m) as [Hpm | Hnpm]; simpl; try (split; reflexivity || assumption)
+    ; destruct (transition l (s2 j, Some (exist proto_message_prop m Hpm))) as [sj' om']
+    ) || destruct (transition l (s2 j, None)) as  [sj' om']
+  ; simpl; split; try reflexivity
+  ;  unfold state_update
+  ;  destruct (eq_dec j j); try contradiction
+  ;  reflexivity
+  .
+Qed.
+
+
+Lemma indexed_transition_projection_state_preservation
+  {oindex : Set} {message : Type} `{Heqd : EqDec oindex}
+  {IS : oindex -> LSM_sig message}
+  {IM : forall i : oindex, @VLSM message (IS i)}
+  {Hinh : inhabited oindex}
+  (s : indexed_state IS)
+  (om : option (indexed_proto_message IS))
+  (l : indexed_label IS)
+  (i : oindex)
+  (Hnli : indexed_ilabel l <> i)
+  : let (s', _) := @transition _ _ (indexed_vlsm IM Hinh) l (s, om) in
+    @indexed_istate_proj _ _ _ _ Hinh i s' = @indexed_istate_proj _ _ _ _ Hinh i s
+  .
+Proof.
   destruct l as [j l]. simpl in Hnli.
   simpl.
   destruct om as [[m Hm]|]
-  ; (destruct (proto_message_decidable m) as [Hpm | Hnpm]; simpl; try reflexivity
-    ; remember (transition l (s j, Some (exist proto_message_prop m Hpm))) as t)
-    || remember (transition l (s j, None)) as t
-  ; destruct t as [s' om']; simpl
-  ; unfold indexed_vlsm_istate_proj
-  ; destruct (eq_dec i j); try (subst; contradiction)
+  ; ( destruct (proto_message_decidable m) as [Hpm | Hnpm]; try reflexivity
+      ; destruct (transition l (s j, Some (exist proto_message_prop m Hpm))) as [s'' om'']
+    ) ||  destruct (transition l (s j, None)) as [s'' om'']
+  ; unfold indexed_istate_proj; unfold state_update
+  ; destruct (eq_dec j i); try contradiction
   ; reflexivity
   .
 Qed.
 
 
-Lemma indexed_vlsm_transition_projection_type_preservation
+Lemma indexed_transition_projection_message_type_mismatch
   {oindex : Set} {message : Type} `{Heqd : EqDec oindex}
-  {IS : oindex -> VLSM message}
-  : forall
-      (s : indexed_state IS)
-      (om : option (indexed_proto_message IS))
-      (l : indexed_label IS)
-      (i : oindex)
-      (Hli : indexed_vlsm_ilabel l = i),
-      noneOrAll
-        (option_map (indexed_vlsm_iproto_message_prop i)
-          (option_map (@proj1_sig message (indexed_proto_message_prop IS))
-            (snd (indexed_transition IS l (s, om)))))
-  .
+  {IS : oindex -> LSM_sig message}
+  {IM : forall i : oindex, @VLSM message (IS i)}
+  {Hinh : inhabited oindex}
+  (s : indexed_state IS)
+  (m : indexed_proto_message IS)
+  (l : indexed_label IS)
+  (i : oindex := indexed_ilabel l)
+  (Hnm : ~ (indexed_iproto_message_prop i (proj1_sig m)))
+  : ~ @valid _ _ (indexed_vlsm IM Hinh)  l (s, Some m) .
 Proof.
-  intros.
-  destruct l as [j l]. simpl in Hli. subst.
-  simpl.
-  destruct om as [[m Hm]|]
-  ; (destruct (proto_message_decidable m) as [Hpm | Hnpm]; simpl; try exact I
-  ; remember (transition l (s i, Some (exist proto_message_prop m Hpm))) as t)
-    || remember (transition l (s i, None)) as t
-  ; destruct t as [s' om']; simpl
-  ; destruct om' as [[m' Hm']|]; simpl; try exact I
-  ;  assumption.
+  simpl. destruct l as [j l]. simpl in i. unfold i in *.
+  destruct m as [m Hm]; simpl in Hnm.
+  destruct (proto_message_decidable m)
+  ; intro; contradiction
+  .
+Qed.
+
+
+Lemma indexed_transition_projection_message_type_preservation
+  {oindex : Set} {message : Type} `{Heqd : EqDec oindex}
+  {IS : oindex -> LSM_sig message}
+  {IM : forall i : oindex, @VLSM message (IS i)}
+  {Hinh : inhabited oindex}
+  (s : indexed_state IS)
+  (om : option (indexed_proto_message IS))
+  (l : indexed_label IS)
+  (i : oindex := indexed_ilabel l)
+  (s' : indexed_state IS)
+  (m' : indexed_proto_message IS)
+  (Ht : @transition _ _ (indexed_vlsm IM Hinh) l (s, om) = (s', Some m'))
+  : indexed_iproto_message_prop i (proj1_sig m').
+Proof.
+  destruct l as [j l]. simpl in i. unfold i in *.
+  unfold indexed_iproto_message_prop.
+  simpl in Ht.
+  destruct om as [[m Hm]|].
+  - destruct (proto_message_decidable m) as [Hpm | Hnpm]
+    ; try destruct (transition l (s j, Some (exist proto_message_prop m Hpm))) as [si' [[m'' Hm'']|]]
+    ; simpl in Ht; inversion Ht; subst; clear Ht.
+    assumption.
+  - destruct (transition l (s j, None)) as [si' [[m'' Hm'']|]]
+    ; simpl in Ht; inversion Ht; subst; clear Ht.
+    assumption.
 Qed.
 
 Definition indexed_vlsm_composed_instance
   {oindex : Set} {message : Type} `{Heqd : EqDec oindex}
-  {IS : oindex -> VLSM message}
-  {Hi : inhabited oindex}
-  : @composed_vlsm_class message (indexed_vlsm IS Hi) :=
-  {| index := oindex
-  ; iproto_state := @indexed_vlsm_istate oindex message Heqd IS
-  ; istate_proj := @indexed_vlsm_istate_proj' oindex message Heqd IS Hi
-  ; ilabel := indexed_vlsm_ilabel
-  ; ilabel_type_inhabited := indexed_vlsm_ilabel_type_inhabited
-  ; iproto_message_prop := indexed_vlsm_iproto_message_prop
-  ; iproto_message_decidable := indexed_vlsm_iproto_message_decidable
-  ; iproto_message_inhabited := indexed_vlsm_iproto_message_inhabited
-  ; iproto_message_consistent := indexed_vlsm_iproto_message_consistent
-  ; transition_projection_consistency := indexed_vlsm_transition_projection_consistency
-  ; transition_projection_state_preservation := indexed_vlsm_transition_projection_state_preservation
-  ; transition_projection_type_preservation := indexed_vlsm_transition_projection_type_preservation
+  {IS : oindex -> LSM_sig message}
+  (IM : forall i : oindex, @VLSM message (IS i))
+  (Hinh : inhabited oindex)
+  : @composed_vlsm_class message _ (indexed_sig_composed_instance IS Hinh) (indexed_vlsm IM Hinh) :=
+  {|  transition_projection_consistency := indexed_transition_projection_consistency
+  ;   transition_projection_state_preservation := indexed_transition_projection_state_preservation
+  ;   transition_projection_message_type_mismatch := indexed_transition_projection_message_type_mismatch
+  ; transition_projection_message_type_preservation := indexed_transition_projection_message_type_preservation
   |}.
 
-Definition indexed_vlsm_constrained_istate_proj
-  {oindex : Set} {message : Type} `{Heqd : EqDec oindex}
-  {IS : oindex -> VLSM message}
-  {Hi : inhabited oindex}
-  (constraint : indexed_label IS -> indexed_state IS * option (indexed_proto_message IS) -> Prop)
-  (i : oindex)
-  (s : @state _ (indexed_vlsm_constrained IS Hi constraint))
-  : @indexed_vlsm_istate oindex message Heqd IS i
-  :=
-  indexed_vlsm_istate_proj i s.
 
-Definition indexed_vlsm_constrained_composed_instance
-  {oindex : Set} {message : Type} `{Heqd : EqDec oindex}
-  (IS : oindex -> VLSM message)
-  (Hi : inhabited oindex)
-  (constraint : indexed_label IS -> indexed_state IS * option (indexed_proto_message IS) -> Prop)
-  : @composed_vlsm_class message (indexed_vlsm_constrained IS Hi constraint) :=
-  {| index := oindex
-  ; iproto_state := @indexed_vlsm_istate oindex message Heqd IS
-  ; istate_proj := @indexed_vlsm_constrained_istate_proj oindex message Heqd IS Hi constraint
-  ; ilabel := indexed_vlsm_ilabel
-  ; ilabel_type_inhabited := indexed_vlsm_ilabel_type_inhabited
-  ; iproto_message_prop := indexed_vlsm_iproto_message_prop
-  ; iproto_message_decidable := indexed_vlsm_iproto_message_decidable
-  ; iproto_message_inhabited := indexed_vlsm_iproto_message_inhabited
-  ; iproto_message_consistent := indexed_vlsm_iproto_message_consistent
-  ; transition_projection_consistency := indexed_vlsm_transition_projection_consistency
-  ; transition_projection_state_preservation := indexed_vlsm_transition_projection_state_preservation
-  ; transition_projection_type_preservation := indexed_vlsm_transition_projection_type_preservation
-  |}.
