indexed_vlsm.v
@@ -1,3 +1,5 @@
+Require Import Logic.FunctionalExtensionality.
+
 
 Require Import ClassicalDescription ClassicalChoice ChoiceFacts.
 
@@ -12,20 +14,20 @@ Assumes classical logic (excluded middle) and the axiom of choice.
 
 Definition indexed_state
   {index : Set} {message : Type}
-  (IS : index -> VLSM message)
+  (IS : index -> LSM_sig message)
   : Type
   :=
   forall i : index, (@state _ (IS i)).
 
 Definition indexed_label
   {index : Set} {message : Type}
-  (IS : index -> VLSM message)
+  (IS : index -> LSM_sig message)
   : Type
   := sigT (fun i => @label _ (IS i)).
 
 Definition indexed_proto_message_prop
   {index : Set} {message : Type}
-  (IS : index -> VLSM message)
+  (IS : index -> LSM_sig message)
   (m : message)
   : Prop
   :=
@@ -33,7 +35,7 @@ Definition indexed_proto_message_prop
 
 Lemma indexed_proto_message_decidable
   {index : Set} {message : Type}
-  (IS : index -> VLSM message)
+  (IS : index -> LSM_sig message)
   : forall m : message, {indexed_proto_message_prop IS m} + {~indexed_proto_message_prop IS m}.
 Proof.
   intros.
@@ -42,12 +44,12 @@ Qed.
 
 Definition indexed_proto_message
   {index : Set} {message : Type}
-  (IS : index -> VLSM message)
+  (IS : index -> LSM_sig message)
   := { m : message | indexed_proto_message_prop IS m }.
 
 Definition indexed_initial_state_prop
   {index : Set} {message : Type}
-  (IS : index -> VLSM message)
+  (IS : index -> LSM_sig message)
   (s : indexed_state IS)
   : Prop
   :=
@@ -55,12 +57,12 @@ Definition indexed_initial_state_prop
 
 Definition indexed_initial_state
   {index : Set} {message : Type}
-  (IS : index -> VLSM message)
+  (IS : index -> LSM_sig message)
   := { s : indexed_state IS | indexed_initial_state_prop IS s }.
 
 Lemma indexed_protocol_state_inhabited
   {index : Set} {message : Type}
-  (IS : index -> VLSM message)
+  (IS : index -> LSM_sig message)
   : inhabited (indexed_initial_state IS).
 Proof.
   unfold indexed_initial_state. unfold indexed_state. unfold indexed_initial_state_prop.
@@ -75,7 +77,7 @@ Qed.
 
 Definition indexed_initial_message_prop
   {index : Set} {message : Type}
-  (IS : index -> VLSM message)
+  (IS : index -> LSM_sig message)
   (m : indexed_proto_message IS)
   : Prop
   :=
@@ -84,7 +86,7 @@ Definition indexed_initial_message_prop
 
 Lemma indexed_message_inhabited
   {index : Set} {message : Type}
-  (IS : index -> VLSM message)
+  (IS : index -> LSM_sig message)
   (Hi : inhabited index)
   : inhabited (indexed_proto_message IS)
   .
@@ -96,7 +98,7 @@ Qed.
 
 Lemma indexed_label_inhabited
   {index : Set} {message : Type}
-  (IS : index -> VLSM message)
+  (IS : index -> LSM_sig message)
   (Hi : inhabited index)
   : inhabited (indexed_label IS).
 Proof.
@@ -109,7 +111,7 @@ Qed.
 
 Definition lift_proto_messageI
   {index : Set} {message : Type}
-  (IS : index -> VLSM message)
+  (IS : index -> LSM_sig message)
   (i : index)
   (mi : @proto_message _ (IS i))
   : indexed_proto_message IS.
@@ -117,38 +119,95 @@ destruct mi as [m Hm].
 exists m. exists i. assumption.
 Defined.
 
+
+Definition indexed_sig
+  {index : Set} {message : Type} `{Heqd : EqDec index}
+  (IS : index -> LSM_sig message)
+  (Hi : inhabited index)
+  : LSM_sig message
+  :=
+  {| state := indexed_state IS
+  ; label := indexed_label IS
+  ; proto_message_prop := indexed_proto_message_prop IS
+  ; proto_message_decidable := indexed_proto_message_decidable IS
+  ; initial_state_prop := indexed_initial_state_prop IS
+  ; protocol_state_inhabited := indexed_protocol_state_inhabited IS
+  ; initial_message_prop := indexed_initial_message_prop IS
+  ; message_inhabited := indexed_message_inhabited IS Hi
+  ; label_inhabited := indexed_label_inhabited IS Hi
+  |}.
+
+Definition state_update
+  {index : Set} {message : Type} `{Heqd : EqDec index}
+  {IS : index -> LSM_sig message}
+  {Hi : inhabited index}
+  (s : @state message (indexed_sig IS Hi))
+  (i : index)
+  (si : @state message (IS i))
+  (j : index)
+  : @state message (IS j).
+destruct (eq_dec i j); subst.
+- exact si.
+- exact (s j).
+Defined.
+
+Definition indexed_ptransition
+  {index : Set} {message : Type} `{Heqd : EqDec index}
+  {IS : index -> LSM_sig message}
+  (IM : forall i : index, @PLSM message (IS i))
+  (Hi : inhabited index)
+  (l : @label message (indexed_sig IS Hi))
+  (som : @state message (indexed_sig IS Hi) * option (@proto_message _ (indexed_sig IS Hi)))
+  : option (@state message (indexed_sig IS Hi) * option (@proto_message _ (indexed_sig IS Hi))).
+destruct l as [i li].
+destruct som as [s [[m Hm]|]].
+- destruct (@proto_message_decidable _ (IS i) m) as [Him | _].
+  + destruct (ptransition li (s i, Some (exist _ m Him))) as [[si' om']|].
+    * exact (Some (state_update s i si', option_map (lift_proto_messageI IS i) om')).
+    * exact None.
+  + exact None.
+- destruct (ptransition li (s i, None)) as [[si' om']|].
+  + exact (Some (state_update s i si', option_map (lift_proto_messageI IS i) om')).
+  + exact None.
+Defined.
+
+Definition indexed_plsm
+  {index : Set} {message : Type} `{Heqd : EqDec index}
+  {IS : index -> LSM_sig message}
+  (IM : forall i : index, @PLSM message (IS i))
+  (Hi : inhabited index)
+  : @PLSM message (indexed_sig IS Hi)
+  :=
+  {|  ptransition := indexed_ptransition IM Hi
+  |}.
+
+
 Definition indexed_transition
   {index : Set} {message : Type} `{Heqd : EqDec index}
-  (IS : index -> VLSM message)
-  (l : indexed_label IS)
-  (som : indexed_state IS * option (indexed_proto_message IS))
-  : indexed_state IS * option (indexed_proto_message IS).
+  {IS : index -> LSM_sig message}
+  (IM : forall i : index, @VLSM message (IS i))
+  (Hinh : inhabited index)
+  (l : @label _ (indexed_sig IS Hinh))
+  (som : @state _ (indexed_sig IS Hinh) * option (@proto_message _ (indexed_sig IS Hinh)))
+  : @state _ (indexed_sig IS Hinh) * option (@proto_message _ (indexed_sig IS Hinh)).
 destruct som as [s om].
 destruct l as [i li].
 destruct om as [[m _]|].
 - destruct (@proto_message_decidable _ (IS i) m) as [Hi | _].
-  + remember (transition li (s i, Some (exist _ m Hi))) as som'.
-    destruct som' as [si' om'].
-    split.
-    * intros j. destruct (eq_dec j i).
-      { subst. exact si' . }
-      exact (s j).
-    * exact (option_map (lift_proto_messageI IS i) om').
+  + destruct (transition li (s i, Some (exist _ m Hi))) as [si' om'].
+    exact (state_update s i si', option_map (lift_proto_messageI IS i) om').
   + exact (s, None).
-- remember (transition li (s i, None)) as som'.
-    destruct som' as [si' om'].
-    split.
-    * intros j. destruct (eq_dec j i).
-      { subst. exact si'. }
-      exact (s j).
-    * exact (option_map (lift_proto_messageI IS i) om').
+- destruct (transition li (s i, None)) as [si' om'].
+    exact (state_update s i si', option_map (lift_proto_messageI IS i) om').
 Defined.
 
 Definition indexed_valid
   {index : Set} {message : Type} `{Heqd : EqDec index}
-  (IS : index -> VLSM message)
-  (l : indexed_label IS)
-  (som : indexed_state IS * option (indexed_proto_message IS))
+  {IS : index -> LSM_sig message}
+  (IM : forall i : index, @VLSM message (IS i))
+  (Hinh : inhabited index)
+  (l : @label _ (indexed_sig IS Hinh))
+  (som : @state _ (indexed_sig IS Hinh) * option (@proto_message _ (indexed_sig IS Hinh)))
   : Prop.
 destruct som as [s om].
 destruct l as [i li].
@@ -159,100 +218,209 @@ destruct om as [[m _]|].
 - exact (valid li (s i, None)).
 Defined.
 
-
-Definition indexed_valid_constrained
-  {index : Set} {message : Type} `{Heqd : EqDec index}
-  (IS : index -> VLSM message)
-  (constraint : indexed_label IS -> indexed_state IS * option (indexed_proto_message IS) -> Prop)
-  (l : indexed_label IS)
-  (som : indexed_state IS * option (indexed_proto_message IS))
-  :=
-  indexed_valid IS l som /\ constraint l som.
-
-
 (* Free VLSM composition *)
 
 Definition indexed_vlsm
   {index : Set} {message : Type} `{Heqd : EqDec index}
-  (IS : index -> VLSM message)
+  {IS : index -> LSM_sig message}
+  (IM : forall i : index, @VLSM message (IS i))
   (Hi : inhabited index)
-  : VLSM message
+  : @VLSM message (indexed_sig IS Hi)
   :=
-  {| state := indexed_state IS
-  ; label := indexed_label IS
-  ; proto_message_prop := indexed_proto_message_prop IS
-  ; proto_message_decidable := indexed_proto_message_decidable IS
-  ; initial_state_prop := indexed_initial_state_prop IS
-  ; protocol_state_inhabited := indexed_protocol_state_inhabited IS
-  ; initial_message_prop := indexed_initial_message_prop IS
-  ; message_inhabited := indexed_message_inhabited IS Hi
-  ; label_inhabited := indexed_label_inhabited IS Hi
-  ; transition := indexed_transition IS
-  ; valid := indexed_valid IS
+  {|  transition := indexed_transition IM Hi
+  ;   valid := indexed_valid IM Hi
   |}.
 
-(* 
-Lemma indexed_valid_decidable
+Definition indexed_valid_decidable
   {index : Set} {message : Type} `{Heqd : EqDec index}
-  (IS : index -> VLSM message)
-  : forall (l : indexed_label IS) (som : indexed_state IS * option (indexed_proto_message IS)),
-  {indexed_valid IS l som} + {~indexed_valid IS l som}.
-Proof.
-  destruct som as [s om].
-  destruct l as [i li]; simpl.
-  destruct om as [[m _]|]; simpl.
-  - destruct (@proto_message_decidable _ (IS i) m) as [Hi | _].
-    + apply valid_decidable.
-    + right; intro; contradiction.
-  - apply valid_decidable.
-Qed.
+  {IS : index -> LSM_sig message}
+  {IM : forall i : index, @VLSM message (IS i)}
+  (IDM : forall i : index, @VLSM_vdecidable _ _ (IM i))
+  (Hinh : inhabited index)
+  (l : @label _ (indexed_sig IS Hinh))
+  (som : @state _ (indexed_sig IS Hinh) * option (@proto_message _ (indexed_sig IS Hinh)))
+  : {@valid _ _ (indexed_vlsm IM Hinh) l som} + {~@valid _ _ (indexed_vlsm IM Hinh) l som}.
+destruct som as [s om].
+destruct l as [i li]; simpl.
+destruct om as [[m _]|]; simpl.
+- destruct (@proto_message_decidable _ (IS i) m) as [Hi | _].
+  + apply valid_decidable.
+  + right; intro; contradiction.
+- apply valid_decidable.
+Defined.
 
-  ; valid_decidable := indexed_valid_decidable IS
+Definition indexed_vlsm_vdecidable
+  {index : Set} {message : Type} `{Heqd : EqDec index}
+  {IS : index -> LSM_sig message}
+  {IM : forall i : index, @VLSM message (IS i)}
+  (IDM : forall i : index, @VLSM_vdecidable _ _ (IM i))
+  (Hi : inhabited index)
+  : @VLSM_vdecidable _ _ (indexed_vlsm IM Hi)
+  :=
+  {|  valid_decidable := indexed_valid_decidable IDM Hi
+  |}.
 
- *)
+Definition indexed_ptransition_constrained
+  {index : Set} {message : Type} `{Heqd : EqDec index}
+  {IS : index -> LSM_sig message}
+  (IM : forall i : index, @PLSM message (IS i))
+  (Hinh : inhabited index)
+  {constraint : @label _ (indexed_sig IS Hinh) -> @state _ (indexed_sig IS Hinh) * option (@proto_message _ (indexed_sig IS Hinh)) -> Prop}
+  (constraint_decidable : forall (l : @label _ (indexed_sig IS Hinh)) (som : @state _ (indexed_sig IS Hinh) * option (@proto_message _ (indexed_sig IS Hinh))), {constraint l som} + {~constraint l som})
+  (l : @label message (indexed_sig IS Hinh))
+  (som : @state message (indexed_sig IS Hinh) * option (@proto_message _ (indexed_sig IS Hinh)))
+  : option (@state message (indexed_sig IS Hinh) * option (@proto_message _ (indexed_sig IS Hinh)))
+  :=
+  if constraint_decidable l som then indexed_ptransition IM Hinh l som else None.
+
+Definition indexed_plsm_constrained
+  {index : Set} {message : Type} `{Heqd : EqDec index}
+  {IS : index -> LSM_sig message}
+  (IM : forall i : index, @PLSM message (IS i))
+  (Hinh : inhabited index)
+  {constraint : @label _ (indexed_sig IS Hinh) -> @state _ (indexed_sig IS Hinh) * option (@proto_message _ (indexed_sig IS Hinh)) -> Prop}
+  (constraint_decidable : forall (l : @label _ (indexed_sig IS Hinh)) (som : @state _ (indexed_sig IS Hinh) * option (@proto_message _ (indexed_sig IS Hinh))), {constraint l som} + {~constraint l som})
+  : @PLSM message (indexed_sig IS Hinh)
+  :=
+  {|  ptransition := indexed_ptransition_constrained IM Hinh constraint_decidable
+  |}.
+
+Definition indexed_valid_constrained
+  {index : Set} {message : Type} `{Heqd : EqDec index}
+  {IS : index -> LSM_sig message}
+  (IM : forall i : index, @VLSM message (IS i))
+  (Hinh : inhabited index)
+  (constraint : indexed_label IS -> indexed_state IS * option (indexed_proto_message IS) -> Prop)
+  (l : @label _ (indexed_sig IS Hinh))
+  (som : @state _ (indexed_sig IS Hinh) * option (@proto_message _ (indexed_sig IS Hinh)))
+  :=
+  indexed_valid IM Hinh l som /\ constraint l som.
+
 
 (* Constrained VLSM composition *)
 
 Definition indexed_vlsm_constrained
   {index : Set} {message : Type} `{Heqd : EqDec index}
-  (IS : index -> VLSM message)
+  {IS : index -> LSM_sig message}
+  (IM : forall i : index, @VLSM message (IS i))
   (Hi : inhabited index)
   (constraint : indexed_label IS -> indexed_state IS * option (indexed_proto_message IS) -> Prop)
-  : VLSM message
+  : @VLSM message (indexed_sig IS Hi)
   :=
-  {| state := indexed_state IS
-  ; label := indexed_label IS
-  ; proto_message_prop := indexed_proto_message_prop IS
-  ; proto_message_decidable := indexed_proto_message_decidable IS
-  ; initial_state_prop := indexed_initial_state_prop IS
-  ; protocol_state_inhabited := indexed_protocol_state_inhabited IS
-  ; initial_message_prop := indexed_initial_message_prop IS
-  ; message_inhabited := indexed_message_inhabited IS Hi
-  ; label_inhabited := indexed_label_inhabited IS Hi
-  ; transition := indexed_transition IS
-  ; valid := indexed_valid_constrained IS constraint
+  {|  transition := indexed_transition IM Hi
+  ;   valid := indexed_valid_constrained IM Hi constraint
   |}.
-
-(* 
 
 Definition indexed_valid_constrained_decidable
   {index : Set} {message : Type} `{Heqd : EqDec index}
-  (IS : index -> VLSM message)
+  {IS : index -> LSM_sig message}
+  {IM : forall i : index, @VLSM message (IS i)}
+  (IDM : forall i : index, @VLSM_vdecidable _ _ (IM i))
+  (Hinh : inhabited index)
   {constraint : indexed_label IS -> indexed_state IS * option (indexed_proto_message IS) -> Prop}
   (constraint_decidable : forall (l : indexed_label IS) (som : indexed_state IS * option (indexed_proto_message IS)), {constraint l som} + {~constraint l som})
-  : forall (l : indexed_label IS) (som : indexed_state IS * option (indexed_proto_message IS)),
-  {indexed_valid_constrained IS constraint l som} + {~indexed_valid_constrained IS constraint l som}.
+  (l : @label _ (indexed_sig IS Hinh))
+  (som : @state _ (indexed_sig IS Hinh) * option (@proto_message _ (indexed_sig IS Hinh)))
+  : {@valid _ _ (indexed_vlsm_constrained IM Hinh constraint) l som} + {~@valid _ _ (indexed_vlsm_constrained IM Hinh constraint) l som}.
+intros.
+unfold indexed_valid_constrained.
+destruct (constraint_decidable l som) as [Hc | Hnc].
+- destruct (indexed_valid_decidable IDM Hinh l som) as [Hv | Hnv].
+  + left. split; try assumption.
+  + right. intros [Hv _]. contradiction.
+- right. intros [_ Hc]. contradiction.
+Defined.
+
+Definition indexed_vlsm_constrained_vdecidable
+  {index : Set} {message : Type} `{Heqd : EqDec index}
+  {IS : index -> LSM_sig message}
+  {IM : forall i : index, @VLSM message (IS i)}
+  (IDM : forall i : index, @VLSM_vdecidable _ _ (IM i))
+  (Hinh : inhabited index)
+  {constraint : indexed_label IS -> indexed_state IS * option (indexed_proto_message IS) -> Prop}
+  (constraint_decidable : forall (l : indexed_label IS) (som : indexed_state IS * option (indexed_proto_message IS)), {constraint l som} + {~constraint l som})
+  : @VLSM_vdecidable _ _ (indexed_vlsm_constrained IM Hinh constraint)
+  :=
+  {|  valid_decidable := indexed_valid_constrained_decidable IDM Hinh constraint_decidable
+  |}.
+
+
+Lemma indexed_partial_composition_commute
+  {index : Set} {message : Type} `{Heqd : EqDec index}
+  {IS : index -> LSM_sig message}
+  {IM : forall i : index, @VLSM message (IS i)}
+  (IDM : forall i : index, @VLSM_vdecidable _ _ (IM i))
+  (Hinh : inhabited index)
+  : let PM12 := DVLSM_PLSM_instance (indexed_vlsm_vdecidable IDM Hinh) in
+    let PM12' := indexed_plsm (fun (i : index) => DVLSM_PLSM_instance (IDM i)) Hinh in
+    @ptransition _ _ PM12 = @ptransition _ _ PM12'.
 Proof.
   intros.
-  unfold indexed_valid_constrained.
-  destruct (constraint_decidable l som) as [Hc | Hnc].
-  - destruct (indexed_valid_decidable IS l som) as [Hv | Hnv].
-    + left. split; try assumption.
-    + right. intros [Hv _]. contradiction.
-  - right. intros [_ Hc]. contradiction.
+  apply functional_extensionality; intros [i li]; apply functional_extensionality; intros [s [[m Hm]|]]
+  ; unfold ptransition; simpl
+  ; unfold transition_valid_ptransition 
+  ; unfold valid_decidable; simpl
+  ; try destruct (proto_message_decidable m) as [Hpm | Hnpm]; try reflexivity
+  ; destruct (IDM i) as [valid_decidablei]; simpl
+  ; try destruct (transition li (s i, Some (exist proto_message_prop m Hpm))) as [si' om']
+  ; try destruct (transition li (s i, None)) as [si' om']
+  .
+  - destruct (valid_decidablei li (s i, Some (exist proto_message_prop m Hpm))) as [Hv | Hnv]
+    ; reflexivity
+    .
+  - destruct (valid_decidablei li (s i, None)) as [Hv | Hnv]
+    ; reflexivity
+    .
 Qed.
 
-  (constraint_decidable : forall (l : indexed_label IS) (som : indexed_state IS * option (indexed_proto_message IS)), {constraint l som} + {~constraint l som})
-  ; valid_decidable := indexed_valid_constrained_decidable IS constraint_decidable
 
- *)
+Lemma indexed_constrained_partial_composition_commute
+  {index : Set} {message : Type} `{Heqd : EqDec index}
+  {IS : index -> LSM_sig message}
+  {IM : forall i : index, @VLSM message (IS i)}
+  (IDM : forall i : index, @VLSM_vdecidable _ _ (IM i))
+  (Hinh : inhabited index)
+  {constraint : @label _ (indexed_sig IS Hinh) -> @state _ (indexed_sig IS Hinh) * option (@proto_message _ (indexed_sig IS Hinh)) -> Prop}
+  (constraint_decidable : forall (l : @label _ (indexed_sig IS Hinh)) (som : @state _ (indexed_sig IS Hinh) * option (@proto_message _ (indexed_sig IS Hinh))), {constraint l som} + {~constraint l som})
+  : let PM12 := DVLSM_PLSM_instance (indexed_vlsm_constrained_vdecidable IDM Hinh constraint_decidable) in
+    let PM12' := indexed_plsm_constrained (fun (i : index) => DVLSM_PLSM_instance (IDM i)) Hinh constraint_decidable in
+    @ptransition _ _ PM12 = @ptransition _ _ PM12'.
+Proof.
+  intros.
+  apply functional_extensionality; intros [i li]; apply functional_extensionality; intros [s [[m Hm]|]]
+  ; unfold ptransition; simpl
+  ; unfold transition_valid_ptransition
+  ; unfold indexed_ptransition_constrained; simpl
+  ; unfold valid_decidable; simpl 
+  ; unfold indexed_valid_constrained_decidable; simpl
+  ; unfold indexed_valid_constrained; simpl
+  ; unfold transition_valid_ptransition; simpl
+  ; unfold valid_decidable
+  ; destruct (IDM i) as [valid_decidablei]
+  .
+  - destruct (constraint_decidable (@existT index (fun i0 : index => @label message (IS i0)) i li)
+        (@pair (@indexed_state index message IS) (option (@proto_message message (@indexed_sig index message Heqd IS Hinh))) s
+           (@Some (@proto_message message (@indexed_sig index message Heqd IS Hinh))
+              (@exist message (fun m0 : message => @indexed_proto_message_prop index message IS m0) m Hm)))
+      )
+    ; try reflexivity
+    .
+    try destruct (proto_message_decidable m) as [Hpm | Hnpm]
+    ; try reflexivity
+    .
+    destruct (transition li (s i, Some (exist proto_message_prop m Hpm))) as [si' om'].
+    destruct (valid_decidablei li (s i, Some (exist proto_message_prop m Hpm)))
+    ; reflexivity
+    .
+  - destruct
+      (constraint_decidable (@existT index (fun i0 : index => @label message (IS i0)) i li)
+        (@pair (@indexed_state index message IS) (option (@proto_message message (@indexed_sig index message Heqd IS Hinh))) s
+           (@None (@proto_message message (@indexed_sig index message Heqd IS Hinh))))
+      )
+    ; try reflexivity.
+    destruct (transition li (s i, None)) as [si' om'].
+    destruct (valid_decidablei li (s i, None)); reflexivity.
+Qed.
+
+
+
