two_vlsms.v
@@ -1,18 +1,20 @@
+Require Import Logic.FunctionalExtensionality.
+
 From Casper
 Require Import vlsm.
 
 Definition composed2_proto_message_prop
   {message}
-  (S1 : VLSM message)
-  (S2 : VLSM message)
+  (S1 : LSM_sig message)
+  (S2 : LSM_sig message)
   (m : message) : Prop
   :=
   (@proto_message_prop _ S1 m) \/ (@proto_message_prop _ S2 m).
 
 Lemma composed2_proto_message_decidable
   {message}
-  (S1 : VLSM message)
-  (S2 : VLSM message)
+  (S1 : LSM_sig message)
+  (S2 : LSM_sig message)
   : forall m : message, {composed2_proto_message_prop S1 S2 m} + {~ composed2_proto_message_prop S1 S2 m}.
 Proof.
   intros.
@@ -25,15 +27,15 @@ Qed.
 
 Definition composed2_proto_message
   {message}
-  (S1 : VLSM message)
-  (S2 : VLSM message)
+  (S1 : LSM_sig message)
+  (S2 : LSM_sig message)
   :=
   { m : message | composed2_proto_message_prop S1 S2 m }.
 
 Definition composed2_initial_state_prop
   {message}
-  (S1 : VLSM message)
-  (S2 : VLSM message)
+  (S1 : LSM_sig message)
+  (S2 : LSM_sig message)
   (s : (@state message S1) * (@state message S2)) : Prop
   :=
   match s with
@@ -42,15 +44,15 @@ Definition composed2_initial_state_prop
 
 Definition composed2_initial_state
   {message}
-  (S1 : VLSM message)
-  (S2 : VLSM message)
+  (S1 : LSM_sig message)
+  (S2 : LSM_sig message)
   :=
   { s : (@state message S1) * (@state message S2) | composed2_initial_state_prop S1 S2 s }.
 
 Lemma composed2_protocol_state_inhabited
   {message}
-  (S1 : VLSM message)
-  (S2 : VLSM message)
+  (S1 : LSM_sig message)
+  (S2 : LSM_sig message)
   : inhabited (composed2_initial_state S1 S2).
 Proof.
   destruct (@protocol_state_inhabited message S1) as [s1].
@@ -61,8 +63,8 @@ Qed.
 
 Definition composed2_initial_message_prop
   {message}
-  (S1 : VLSM message)
-  (S2 : VLSM message)
+  (S1 : LSM_sig message)
+  (S2 : LSM_sig message)
   (m : composed2_proto_message S1 S2) : Prop.
 destruct m as [m Hm].
 destruct (@proto_message_decidable _ S1 m) as [H1 | _]; destruct (@proto_message_decidable _ S2 m) as [H2 | _].
@@ -74,8 +76,8 @@ Defined.
 
 Lemma composed2_message_inhabited
   {message}
-  (S1 : VLSM message)
-  (S2 : VLSM message)
+  (S1 : LSM_sig message)
+  (S2 : LSM_sig message)
   : inhabited (composed2_proto_message S1 S2)
   .
 Proof.
@@ -85,8 +87,8 @@ Qed.
 
 Lemma composed2_label_inhabited
   {message}
-  (S1 : VLSM message)
-  (S2 : VLSM message)
+  (S1 : LSM_sig message)
+  (S2 : LSM_sig message)
   : inhabited ((@label message S1) + (@label message S2)).
 Proof.
   destruct (@label_inhabited message S1) as [l].
@@ -96,8 +98,8 @@ Qed.
 
 Definition lift_proto_message1
   {message}
-  (S1 : VLSM message)
-  (S2 : VLSM message)
+  (S1 : LSM_sig message)
+  (S2 : LSM_sig message)
   (m1 : @proto_message _ S1)
   : composed2_proto_message S1 S2.
 destruct m1 as [m1 Hm1].
@@ -108,8 +110,8 @@ Defined.
 
 Definition lift_proto_message2
   {message}
-  (S1 : VLSM message)
-  (S2 : VLSM message)
+  (S1 : LSM_sig message)
+  (S2 : LSM_sig message)
   (m2 : @proto_message _ S2)
   : composed2_proto_message S1 S2.
 destruct m2 as [m2 Hm2].
@@ -117,13 +119,74 @@ exists m2.
 unfold composed2_proto_message_prop. right. assumption.
 Defined.
 
+Definition composed2_sig
+  {message}
+  (S1 : LSM_sig message)
+  (S2 : LSM_sig message)
+  : LSM_sig message
+  :=
+  {| state := (@state message S1) * (@state message S2)
+  ; label := (@label message S1) + (@label message S2)
+  ; proto_message_prop := composed2_proto_message_prop S1 S2
+  ; proto_message_decidable := composed2_proto_message_decidable S1 S2
+  ; initial_state_prop := composed2_initial_state_prop S1 S2
+  ; protocol_state_inhabited := composed2_protocol_state_inhabited S1 S2
+  ; initial_message_prop := composed2_initial_message_prop S1 S2
+  ; message_inhabited := composed2_message_inhabited S1 S2
+  ; label_inhabited := composed2_label_inhabited S1 S2
+  |}.
+
+
+Definition composed2_ptransition
+  {message}
+  {S1 : LSM_sig message}
+  {S2 : LSM_sig message}
+  (M1 : @PLSM message S1)
+  (M2 : @PLSM message S2)
+  (l : @label message (composed2_sig S1 S2))
+  (som : @state message (composed2_sig S1 S2) * option (@proto_message _ (composed2_sig S1 S2)))
+  : option (@state message (composed2_sig S1 S2) * option (@proto_message _ (composed2_sig S1 S2))).
+destruct som as [[s1 s2] [[m Hm]|]].
+- destruct l as [l1 | l2].
+  + destruct (@proto_message_decidable _ S1 m) as [H1 | _].
+    * destruct (ptransition l1 (s1, Some (exist _ m H1))) as [som'|].
+      { exact (Some ((fst som', s2), option_map (lift_proto_message1 S1 S2) (snd som'))). }
+      exact None.
+    * exact None.
+  + destruct (@proto_message_decidable _ S2 m) as [H2 | _].
+    * destruct (ptransition l2 (s2, Some (exist _ m H2))) as [som'|].
+      { exact (Some ((s1, fst som'), option_map (lift_proto_message2 S1 S2) (snd som'))). }
+      exact None.
+    * exact None.
+- destruct l as [l1 | l2].
+  + destruct (ptransition l1 (s1, None)) as [som'|].
+    * exact (Some ((fst som', s2), option_map (lift_proto_message1 S1 S2) (snd som'))).
+    * exact None.
+  + destruct (ptransition l2 (s2, None)) as [som'|].
+    * exact (Some ((s1, fst som'), option_map (lift_proto_message2 S1 S2) (snd som'))).
+    * exact None.
+Defined.
+
+Definition composed2_plsm
+  {message}
+  {S1 : LSM_sig message}
+  {S2 : LSM_sig message}
+  (M1 : @PLSM message S1)
+  (M2 : @PLSM message S2)
+  : @PLSM message (composed2_sig S1 S2)
+  :=
+  {|  ptransition := composed2_ptransition M1 M2
+  |}.
+
 Definition composed2_transition
   {message}
-  (S1 : VLSM message)
-  (S2 : VLSM message)
-  (l : (@label message S1) + (@label message S2))
-  (som : ((@state message S1) * (@state message S2)) * option (composed2_proto_message S1 S2))
-  : (((@state message S1) * (@state message S2)) * option (composed2_proto_message S1 S2))%type.
+  {S1 : LSM_sig message}
+  {S2 : LSM_sig message}
+  (M1 : @VLSM message S1)
+  (M2 : @VLSM message S2)
+  (l : @label message (composed2_sig S1 S2))
+  (som : @state message (composed2_sig S1 S2) * option (@proto_message _ (composed2_sig S1 S2)))
+  : @state message (composed2_sig S1 S2) * option (@proto_message _ (composed2_sig S1 S2)).
 destruct som as [[s1 s2] [[m Hm]|]].
 - destruct l as [l1 | l2].
   + destruct (@proto_message_decidable _ S1 m) as [H1 | _].
@@ -143,10 +206,12 @@ Defined.
 
 Definition composed2_valid
   {message}
-  (S1 : VLSM message)
-  (S2 : VLSM message)
-  (l : (@label message S1) + (@label message S2))
-  (som : ((@state message S1) * (@state message S2)) * option (composed2_proto_message S1 S2))
+  {S1 : LSM_sig message}
+  {S2 : LSM_sig message}
+  (M1 : @VLSM message S1)
+  (M2 : @VLSM message S2)
+  (l : @label message (composed2_sig S1 S2))
+  (som : @state message (composed2_sig S1 S2) * option (@proto_message _ (composed2_sig S1 S2)))
   : Prop.
 destruct som as [[s1 s2] [[m Hm]|]].
 - destruct l as [l1 | l2].
@@ -161,44 +226,29 @@ destruct som as [[s1 s2] [[m Hm]|]].
   + exact (valid l2 (s2, None)).
 Defined.
 
-Definition composed2_valid_constrained
-  {message}
-  (S1 : VLSM message)
-  (S2 : VLSM message)
-  (constraint : (@label message S1) + (@label message S2) -> ((@state message S1) * (@state message S2)) * option (composed2_proto_message S1 S2) -> Prop)
-  (l : (@label message S1) + (@label message S2))
-  (som : ((@state message S1) * (@state message S2)) * option (composed2_proto_message S1 S2))
-  :=
-  composed2_valid S1 S2 l som /\ constraint l som.
-
 Definition composed2_vlsm
   {message}
-  (S1 : VLSM message)
-  (S2 : VLSM message)
-  : VLSM message
+  {S1 : LSM_sig message}
+  {S2 : LSM_sig message}
+  (M1 : @VLSM message S1)
+  (M2 : @VLSM message S2)
+  : @VLSM message (composed2_sig S1 S2)
   :=
-  {| state := (@state message S1) * (@state message S2)
-  ; label := (@label message S1) + (@label message S2)
-  ; proto_message_prop := composed2_proto_message_prop S1 S2
-  ; proto_message_decidable := composed2_proto_message_decidable S1 S2
-  ; initial_state_prop := composed2_initial_state_prop S1 S2
-  ; protocol_state_inhabited := composed2_protocol_state_inhabited S1 S2
-  ; initial_message_prop := composed2_initial_message_prop S1 S2
-  ; message_inhabited := composed2_message_inhabited S1 S2
-  ; label_inhabited := composed2_label_inhabited S1 S2
-  ; transition := composed2_transition S1 S2
-  ; valid := composed2_valid S1 S2
+  {|  transition := composed2_transition M1 M2
+  ;   valid := composed2_valid M1 M2
   |}.
 
-Lemma composed2_valid_decidable
+
+Definition composed2_valid_decidable
   {message}
-  {S1 S2 : VLSM message}
-  (DS1 : @VLSM_vdecidable message S1)
-  (DS2 : @VLSM_vdecidable message S2)
-  (l : @label message (composed2_vlsm S1 S2))
-  (som : @state _ (composed2_vlsm S1 S2) * option (@proto_message _ (composed2_vlsm S1 S2)))
-  : {@valid _ (composed2_vlsm S1 S2) l som} + {~@valid _ (composed2_vlsm S1 S2) l som}.
-Proof.
+  {S1 S2 : LSM_sig message}
+  {M1 : @VLSM message S1}
+  {M2 : @VLSM message S2}
+  (DS1 : @VLSM_vdecidable message S1 M1)
+  (DS2 : @VLSM_vdecidable message S2 M2)
+  (l : @label message (composed2_sig S1 S2))
+  (som : @state _ (composed2_sig S1 S2) * option (@proto_message _ (composed2_sig S1 S2)))
+  : {@valid _ _ (composed2_vlsm M1 M2) l som} + {~@valid _ _ (composed2_vlsm M1 M2) l som}.
   destruct som as [[s1 s2] [[m Hm]|]].
   - destruct l as [l1 | l2]; simpl.
     + destruct (@proto_message_decidable _ S1 m) as [H1 | _].
@@ -208,73 +258,189 @@ Proof.
       * apply valid_decidable.
       * right. intro. assumption.
   - destruct l as [l1 | l2]; simpl; apply valid_decidable.
-Qed.
+Defined.
 
 Definition composed2_vlsm_vdecidable
   {message}
-  {S1 S2 : VLSM message}
-  (DS1 : @VLSM_vdecidable message S1)
-  (DS2 : @VLSM_vdecidable message S2)
-  : @VLSM_vdecidable message (composed2_vlsm S1 S2)
+  {S1 S2 : LSM_sig message}
+  {M1 : @VLSM message S1}
+  {M2 : @VLSM message S2}
+  (DS1 : @VLSM_vdecidable message S1 M1)
+  (DS2 : @VLSM_vdecidable message S2 M2)
+  : @VLSM_vdecidable message _ (composed2_vlsm M1 M2)
   :=
   {|
     valid_decidable := composed2_valid_decidable DS1 DS2
   |}.
 
+Definition composed2_ptransition_constrained
+  {message}
+  {S1 : LSM_sig message}
+  {S2 : LSM_sig message}
+  (M1 : @PLSM message S1)
+  (M2 : @PLSM message S2)
+  {constraint : (@label message S1) + (@label message S2) -> ((@state message S1) * (@state message S2)) * option (composed2_proto_message S1 S2) -> Prop}
+  (constraint_decidable : forall (l : (@label message S1) + (@label message S2)) (som : ((@state message S1) * (@state message S2)) * option (composed2_proto_message S1 S2)), {constraint l som} + {~constraint l som})
+  (l : @label message (composed2_sig S1 S2))
+  (som : @state message (composed2_sig S1 S2) * option (@proto_message _ (composed2_sig S1 S2)))
+  : option (@state message (composed2_sig S1 S2) * option (@proto_message _ (composed2_sig S1 S2)))
+  :=
+  if constraint_decidable l som then composed2_ptransition M1 M2 l som else None.
+
+Definition composed2_plsm_constrained
+  {message}
+  {S1 : LSM_sig message}
+  {S2 : LSM_sig message}
+  (M1 : @PLSM message S1)
+  (M2 : @PLSM message S2)
+  {constraint : (@label message S1) + (@label message S2) -> ((@state message S1) * (@state message S2)) * option (composed2_proto_message S1 S2) -> Prop}
+  (constraint_decidable : forall (l : (@label message S1) + (@label message S2)) (som : ((@state message S1) * (@state message S2)) * option (composed2_proto_message S1 S2)), {constraint l som} + {~constraint l som})
+  : @PLSM message (composed2_sig S1 S2)
+  :=
+  {|  ptransition := composed2_ptransition_constrained M1 M2 constraint_decidable
+  |}.
+
+Definition composed2_valid_constrained
+  {message}
+  {S1 : LSM_sig message}
+  {S2 : LSM_sig message}
+  (M1 : @VLSM message S1)
+  (M2 : @VLSM message S2)
+  (constraint : @label message (composed2_sig S1 S2) -> @state message (composed2_sig S1 S2) * option (@proto_message _ (composed2_sig S1 S2)) -> Prop)
+  (l : @label message (composed2_sig S1 S2))
+  (som : @state message (composed2_sig S1 S2) * option (@proto_message _ (composed2_sig S1 S2)))
+  :=
+  composed2_valid M1 M2 l som /\ constraint l som.
 
 Definition composed2_vlsm_constrained
   {message}
-  (S1 : VLSM message)
-  (S2 : VLSM message)
+  {S1 : LSM_sig message}
+  {S2 : LSM_sig message}
+  (M1 : @VLSM message S1)
+  (M2 : @VLSM message S2)
   (constraint : (@label message S1) + (@label message S2) -> (@state message S1 * @state message S2) * option (composed2_proto_message S1 S2) -> Prop)
-  : VLSM message
+  : @VLSM message (composed2_sig S1 S2)
   :=
-  {| state := (@state message S1) * (@state message S2)
-  ; label := (@label message S1) + (@label message S2)
-  ; proto_message_prop := composed2_proto_message_prop S1 S2
-  ; proto_message_decidable := composed2_proto_message_decidable S1 S2
-  ; initial_state_prop := composed2_initial_state_prop S1 S2
-  ; protocol_state_inhabited := composed2_protocol_state_inhabited S1 S2
-  ; initial_message_prop := composed2_initial_message_prop S1 S2
-  ; message_inhabited := composed2_message_inhabited S1 S2
-  ; label_inhabited := composed2_label_inhabited S1 S2
-  ; transition := composed2_transition S1 S2
-  ; valid := composed2_valid_constrained S1 S2 constraint
+  {|  transition := composed2_transition M1 M2
+  ;   valid := composed2_valid_constrained M1 M2 constraint
   |}.
 
-Lemma composed2_constrained_valid_decidable
+Definition composed2_constrained_valid_decidable
   {message}
-  {S1 S2 : VLSM message}
-  (DS1 : @VLSM_vdecidable message S1)
-  (DS2 : @VLSM_vdecidable message S2)
+  {S1 S2 : LSM_sig message}
+  {M1 : @VLSM message S1}
+  {M2 : @VLSM message S2}
+  (DS1 : @VLSM_vdecidable message S1 M1)
+  (DS2 : @VLSM_vdecidable message S2 M2)
   {constraint : (@label message S1) + (@label message S2) -> ((@state message S1) * (@state message S2)) * option (composed2_proto_message S1 S2) -> Prop}
   (constraint_decidable : forall (l : (@label message S1) + (@label message S2)) (som : ((@state message S1) * (@state message S2)) * option (composed2_proto_message S1 S2)), {constraint l som} + {~constraint l som})
-  (l : @label message (composed2_vlsm_constrained S1 S2 constraint))
-  (som : @state _ (composed2_vlsm_constrained S1 S2 constraint) * option (@proto_message _ (composed2_vlsm_constrained S1 S2 constraint)))
-  : {@valid _ (composed2_vlsm_constrained S1 S2 constraint) l som} + {~@valid _ (composed2_vlsm_constrained S1 S2 constraint) l som}.
-Proof.
-  unfold label in l; simpl in l.
-  unfold state in som. unfold proto_message in som. simpl in som.
-  unfold valid; simpl.
-  destruct (constraint_decidable l som) as [Hc | Hnc].
-  - destruct (composed2_valid_decidable DS1 DS2 l som) as [Hv | Hnv].
-    + left. split; try assumption.
-    + right. intros [Hv _]. contradiction.
-  - right. intros [_ Hc]. contradiction.
-Qed.
+  (l : @label message (composed2_sig S1 S2))
+  (som : @state _ (composed2_sig S1 S2) * option (@proto_message _ (composed2_sig S1 S2)))
+  : {@valid _ _ (composed2_vlsm_constrained M1 M2 constraint) l som} + {~@valid _ _ (composed2_vlsm_constrained M1 M2 constraint) l som}.
+unfold label in l; simpl in l.
+unfold state in som. unfold proto_message in som. simpl in som.
+unfold valid; simpl.
+destruct (constraint_decidable l som) as [Hc | Hnc].
+- destruct (composed2_valid_decidable DS1 DS2 l som) as [Hv | Hnv].
+  + left. split; try assumption.
+  + right. intros [Hv _]. contradiction.
+- right. intros [_ Hc]. contradiction.
+Defined.
 
 Definition composed2_vlsm_constrained_vdecidable
   {message}
-  {S1 S2 : VLSM message}
-  (DS1 : @VLSM_vdecidable message S1)
-  (DS2 : @VLSM_vdecidable message S2)
-  (constraint : (@label message S1) + (@label message S2) -> (@state message S1 * @state message S2) * option (composed2_proto_message S1 S2) -> Prop)
+  {S1 S2 : LSM_sig message}
+  {M1 : @VLSM message S1}
+  {M2 : @VLSM message S2}
+  (DS1 : @VLSM_vdecidable message S1 M1)
+  (DS2 : @VLSM_vdecidable message S2 M2)
+  {constraint : (@label message S1) + (@label message S2) -> (@state message S1 * @state message S2) * option (composed2_proto_message S1 S2) -> Prop}
   (constraint_decidable : forall (l : (@label message S1) + (@label message S2)) (som : ((@state message S1) * (@state message S2)) * option (composed2_proto_message S1 S2)), {constraint l som} + {~constraint l som})
-  : @VLSM_vdecidable message (composed2_vlsm_constrained S1 S2 constraint)
+  : @VLSM_vdecidable message _ (composed2_vlsm_constrained M1 M2 constraint)
   :=
   {|
     valid_decidable := composed2_constrained_valid_decidable DS1 DS2 constraint_decidable
   |}.
 
+Lemma composed2_partial_composition_commute
+  {message}
+  {S1 S2 : LSM_sig message}
+  {M1 : @VLSM message S1}
+  {M2 : @VLSM message S2}
+  (DS1 : @VLSM_vdecidable message S1 M1)
+  (DS2 : @VLSM_vdecidable message S2 M2)
+  : let PM12 := DVLSM_PLSM_instance (composed2_vlsm_vdecidable DS1 DS2) in
+    let PM12' := composed2_plsm (DVLSM_PLSM_instance DS1) (DVLSM_PLSM_instance DS2) in
+    @ptransition _ _ PM12 = @ptransition _ _ PM12'.
+Proof.
+  intros.
+  apply functional_extensionality; intros [l1 | l2]; apply functional_extensionality; intros [[s1 s2] [[m Hm]|]];
+  unfold ptransition; simpl;
+  unfold transition_valid_ptransition; unfold valid_decidable; simpl; try destruct (proto_message_decidable m) as [Hpm | Hnpm]; try reflexivity
+  ; destruct DS1 as [valid_decidable1]; destruct DS2 as [valid_decidable2]; simpl
+  .
+  - destruct (valid_decidable1 l1 (s1, Some (exist proto_message_prop m Hpm))) as [Hv | Hnv]; reflexivity.
+  - destruct (valid_decidable1 l1 (s1, None)) as [Hv | Hnv]; reflexivity.
+  - destruct (valid_decidable2 l2 (s2, Some (exist proto_message_prop m Hpm))) as [Hv | Hnv]; reflexivity.
+  - destruct (valid_decidable2 l2 (s2, None)) as [Hv | Hnv]; reflexivity.
+Qed.
 
 
+Lemma composed2_constrained_partial_composition_commute
+  {message}
+  {S1 S2 : LSM_sig message}
+  {M1 : @VLSM message S1}
+  {M2 : @VLSM message S2}
+  (DS1 : @VLSM_vdecidable message S1 M1)
+  (DS2 : @VLSM_vdecidable message S2 M2)
+  {constraint : (@label message S1) + (@label message S2) -> (@state message S1 * @state message S2) * option (composed2_proto_message S1 S2) -> Prop}
+  (constraint_decidable : forall (l : (@label message S1) + (@label message S2)) (som : ((@state message S1) * (@state message S2)) * option (composed2_proto_message S1 S2)), {constraint l som} + {~constraint l som})
+  : let PM12 := DVLSM_PLSM_instance (composed2_vlsm_constrained_vdecidable DS1 DS2 constraint_decidable) in
+    let PM12' := composed2_plsm_constrained (DVLSM_PLSM_instance DS1) (DVLSM_PLSM_instance DS2) constraint_decidable in
+    @ptransition _ _ PM12 = @ptransition _ _ PM12'.
+Proof.
+  intros.
+  apply functional_extensionality; intros [l1 | l2]; apply functional_extensionality; intros [[s1 s2] [[m Hm]|]]
+  ; unfold ptransition; simpl
+  ; unfold transition_valid_ptransition; unfold composed2_ptransition_constrained
+  ; unfold valid_decidable; simpl 
+  ; unfold composed2_constrained_valid_decidable; simpl
+  ; unfold composed2_valid_constrained; simpl
+  ; try destruct
+    (constraint_decidable (@inl (@label message S1) (@label message S2) l1)
+      (s1, s2,
+      @Some (@proto_message message (@composed2_sig message S1 S2))
+        (@exist message
+           (fun m0 : message => @composed2_proto_message_prop message S1 S2 m0) m Hm))
+    )
+  ; try reflexivity
+  ; try destruct
+    (constraint_decidable (@inl (@label message S1) (@label message S2) l1)
+      (s1, s2, @None (@proto_message message (@composed2_sig message S1 S2)))
+    )
+  ; try reflexivity
+  ; try destruct
+    (constraint_decidable (@inr (@label message S1) (@label message S2) l2)
+      (s1, s2,
+      @Some (@proto_message message (@composed2_sig message S1 S2))
+        (@exist message
+           (fun m0 : message => @composed2_proto_message_prop message S1 S2 m0) m Hm))
+    )
+  ; try reflexivity
+  ; try destruct
+    (constraint_decidable (@inr (@label message S1) (@label message S2) l2)
+      (s1, s2, @None (@proto_message message (@composed2_sig message S1 S2)))
+    )
+  ; try reflexivity
+  ; unfold transition_valid_ptransition; simpl
+  ; unfold valid_decidable; destruct DS1 as [valid_decidable1]; destruct DS2 as [valid_decidable2]; simpl
+  ; try destruct (proto_message_decidable m) as [Hpm | Hnpm]
+  ; try reflexivity
+  .
+  - destruct (valid_decidable1 l1 (s1, Some (exist proto_message_prop m Hpm))); reflexivity.
+  - destruct (valid_decidable1 l1 (s1, Some (exist proto_message_prop m Hpm))); reflexivity.
+  - destruct (valid_decidable1 l1 (s1, None)) as [Hv | Hnv]; reflexivity.
+  - destruct (valid_decidable2 l2 (s2, Some (exist proto_message_prop m Hpm))) as [Hv | Hnv]; reflexivity.
+  - destruct (valid_decidable2 l2 (s2, Some (exist proto_message_prop m Hpm))) as [Hv | Hnv]; reflexivity.
+  - destruct (valid_decidable2 l2 (s2, None)) as [Hv | Hnv]; reflexivity.
+Qed.
