vlsm.v
@@ -47,7 +47,7 @@ Qed.
 
 (* 2.2.1 VLSM Parameters *)
 
-Class VLSM (message : Type) :=
+Class LSM_sig (message : Type) :=
   { state : Type
   ; label : Type
   ; proto_message_prop : message -> Prop
@@ -60,13 +60,82 @@ Class VLSM (message : Type) :=
   ; protocol_state_inhabited : inhabited initial_state
   ; message_inhabited : inhabited proto_message
   ; label_inhabited : inhabited label
-  ; transition : label -> state * option proto_message -> state * option proto_message
+  }.
+
+Class PLSM (message : Type) `{Sig : LSM_sig message} :=
+  { ptransition : label -> state * option proto_message -> option (state * option proto_message)
+  }.
+
+Class VLSM (message : Type) `{Sig : LSM_sig message } :=
+  { transition : label -> state * option proto_message -> state * option proto_message
   ; valid : label -> state * option proto_message -> Prop
   }.
+
+
+Definition ptransition_to_transition
+  {message}
+  {Sig : LSM_sig message}
+  `{PM : @PLSM message Sig}
+  (l : label)
+  (som :  state * option proto_message)
+  : state * option proto_message
+  :=
+  match ptransition l som with
+  | Some som' => som'
+  | None => (fst som, None)
+  end
+  .
+
+Definition ptransition_to_valid
+  {message}
+  {Sig : LSM_sig message}
+  `{PM : @PLSM message Sig}
+  (l : label)
+  (som :  state * option proto_message)
+  : Prop
+  :=
+  ptransition l som = None
+  .
+
+Definition PLSM_VLSM_instance
+  {message}
+  {Sig : LSM_sig message}
+  `{PM : @PLSM message Sig}
+  : @VLSM message Sig
+  :=
+  {|  transition := ptransition_to_transition
+  ;   valid := ptransition_to_valid
+  |}.
 
 Class VLSM_vdecidable (message : Type) `{M : VLSM message} :=
   { valid_decidable : forall l som, {valid l som} + {~valid l som} 
   }.
+
+
+Definition transition_valid_ptransition
+  {message}
+  {Sig : LSM_sig message}
+  {VM : @VLSM message Sig}
+  `{DVM : @VLSM_vdecidable message Sig VM}
+  (l : label)
+  (som :  state * option proto_message)
+  : option (state * option proto_message)
+  :=
+  if valid_decidable l som
+  then Some (transition l som)
+  else None
+  .
+
+Definition DVLSM_PLSM_instance
+  {message}
+  {Sig : LSM_sig message}
+  {VM : @VLSM message Sig}
+  `{DVM : @VLSM_vdecidable message Sig VM}
+  : @PLSM message Sig
+  :=
+  {|  ptransition := transition_valid_ptransition
+  |}.
+
 
 (* 2.2.2 VLSM protocol states and protocol messages *)
 
