indexed_vlsm_projections.v
@@ -4,24 +4,30 @@ Require Import vlsm composed_vlsm composed_vlsm_projections indexed_vlsm.
 Definition indexed_vlsm_projection
   {message : Type}
   {oindex : Set} {message : Type} `{Heqd : EqDec oindex}
-  (IS : oindex -> VLSM message)
+  (IS : oindex -> LSM_sig message)
+  (IM : forall i : oindex, @VLSM message (IS i))
   (i : oindex)
   : VLSM (message : Type)
   :=
   @vlsm_projection message
-    (indexed_vlsm IS (inhabits i))
-    (@indexed_vlsm_composed_instance oindex message Heqd IS (inhabits i))
+    (indexed_sig IS (inhabits i))
+    (indexed_sig_composed_instance IS (inhabits i))
+    (indexed_vlsm IM (inhabits i))
+    (@indexed_vlsm_composed_instance oindex message Heqd IS IM (inhabits i))
     i
   .
 
 Definition indexed_vlsm_constrained_projection
   {oindex : Set} {message : Type} `{Heqd : EqDec oindex}
-  (IS : oindex -> VLSM message)
+  (IS : oindex -> LSM_sig message)
+  (IM : forall i : oindex, @VLSM message (IS i))
   (constraint : indexed_label IS -> indexed_state IS * option (indexed_proto_message IS) -> Prop)
   (i : oindex)
   : VLSM (message : Type)
   :=
   @vlsm_projection message
+    (indexed_sig IS (inhabits i))
+    (indexed_sig_composed_instance IS (inhabits i))
     (indexed_vlsm_constrained IS (inhabits i) constraint)
     (@indexed_vlsm_constrained_composed_instance oindex message Heqd IS (inhabits i) constraint)
     i
